.

theories/System/LGS.v
@@ -76,23 +76,21 @@ Module LGS (Token : TOKEN_SPEC).
 
 #[local] Existing Instance Token.t_hasEqDec.
 
-Module Error.
+Module BuildError.
 
 Inductive t : Set :=
-  | NullableTokenRule (idx : nat)
-  | NoMatch (rest : list ascii)
-  | InternalInvariantBroken.
+  | NullableTokenRule (idx : nat).
 
-End Error.
+End BuildError.
 
 #[universes(polymorphic=yes)]
-Definition ErrM@{u | } (A : Type@{u}) : Type@{u} :=
-  Error.t + A.
+Definition BuildErrorM@{u | } (A : Type@{u}) : Type@{u} :=
+  BuildError.t + A.
 
 #[universes(polymorphic=yes)]
-Instance ErrM_isMonad@{u} : isMonad@{u u} ErrM@{u} :=
+Instance ErrM_isMonad@{u} : isMonad@{u u} BuildErrorM@{u} :=
   { pure {A : Type@{u}} (x : A) := inr x
-  ; bind {A : Type@{u}} {B : Type@{u}} (m : ErrM A) (k : A -> ErrM B) := B.either (@inl _ _) k m
+  ; bind {A : Type@{u}} {B : Type@{u}} (m : BuildErrorM A) (k : A -> BuildErrorM B) := B.either (@inl _ _) k m
   }.
 
 Module Input.
@@ -184,6 +182,60 @@ Proof.
   - reflexivity.
 Qed.
 
+Module Rule.
+
+#[projections(primitive)]
+Record t : Set :=
+  mk
+  { index : nat
+  ; token : Token.t
+  ; regex : Re.t ascii
+  }.
+
+#[global]
+Instance Rule_hasEqDec
+  : hasEqDec@{Set} Rule.t.
+Proof.
+  red. decide equality.
+  - eapply eq_dec.
+  - eapply eq_dec.
+  - eapply eq_dec.
+Defined.
+
+Definition compile_rule (rule : Rule.t) : BuildErrorM Rule.t :=
+  if nullable rule.(regex) then
+    inl (BuildError.NullableTokenRule rule.(index))
+  else
+    pure rule.
+
+Theorem compile_rule_spec (rule : Rule.t) (compiled_rule : Rule.t)
+  (COMPILE : compile_rule rule = inr compiled_rule)
+  : forall s, s \in eval_regex rule.(regex) <-> s \in eval_regex compiled_rule.(regex).
+Proof.
+  intros s; split; intros ACCEPTS; unfold compile_rule in COMPILE; now destruct (nullable rule.(regex)) eqn: NULLABLE; inv COMPILE.
+Qed.
+
+Lemma compile_rule_not_match_empty (rule : Rule.t) (compiled_rule : Rule.t)
+  (COMPILE : compile_rule rule = inr compiled_rule)
+  : ~ ([] \in eval_regex compiled_rule.(regex)).
+Proof.
+  unfold compile_rule in COMPILE; destruct (nullable rule.(regex)) eqn: NULLABLE; inv COMPILE; now rewrite <- nullable_false_iff.
+Qed.
+
+Fixpoint compile_rules (rules : list Rule.t) {struct rules} : BuildErrorM (list Rule.t) :=
+  match rules with
+  | [] => pure (@nil Rule.t)
+  | rule :: rules => liftM2 (@cons Rule.t) (compile_rule rule) (compile_rules rules)
+  end.
+
+Definition raws : list Rule.t :=
+  L.mapi_from 1 (fun index => fun '(token, regex) => Rule.mk index token regex) Token.rules.
+
+Definition compileds : BuildErrorM (list Rule.t) :=
+  compile_rules raws.
+
+End Rule.
+
 Module TaggedENFA.
 
 #[projections(primitive)]
@@ -201,7 +253,7 @@ Record t : Type :=
 #[global] Existing Instance state_hasEqDec.
 
 Definition accept_state (M : TaggedENFA.t) : Set :=
-  (M.(state) * Token.t).
+  M.(state) * Token.t.
 
 Variant okay (M : TaggedENFA.t) : Prop :=
   | okay_intro
@@ -210,41 +262,27 @@ Variant okay (M : TaggedENFA.t) : Prop :=
     (eps_step_okay : forall q, forall q', q ∈ M.(states) -> q' ∈ M.(eps_step) q -> q' ∈ M.(states))
     (char_step_okay : forall q, forall q', forall c, q ∈ M.(states) -> q' ∈ M.(char_step) q c -> q' ∈ M.(states)).
 
-Section BASICS.
+Section DELTA_STAR.
 
-Variable M : TaggedENFA.t.
+Context {Q : Type}.
 
-#[local] Notation Q := M.(state).
+Variable eps_step : Q -> list Q.
+
+Variable char_step : Q -> ascii -> list Q.
 
 Inductive delta_star (q : Q) : Input.t -> ensemble Q :=
   | delta_star_nil
     : q \in delta_star q []
   | delta_star_eps q1 q2 s
-    (STEP : q1 ∈ M.(eps_step) q)
+    (STEP : q1 ∈ eps_step q)
     (REST : q2 \in delta_star q1 s)
     : q2 \in delta_star q s
   | delta_star_char q1 q2 c s
-    (STEP : q1 ∈ M.(char_step) q c)
+    (STEP : q1 ∈ char_step q c)
     (REST : q2 \in delta_star q1 s)
     : q2 \in delta_star q (c :: s).
 
 #[local] Hint Constructors delta_star : core.
-
-Inductive eclosure (q : Q) : ensemble Q :=
-  | eclosure_refl
-    : q \in eclosure q
-  | eclosure_step q1 q2
-    (STEP : q1 ∈ M.(eps_step) q)
-    (REST : q2 \in eclosure q1)
-    : q2 \in eclosure q.
-
-#[local] Hint Constructors eclosure : core.
-
-Definition accepts (s : Input.t) (tag : Token.t) : Prop :=
-  exists q, q \in delta_star M.(start_state) s /\ (q, tag) ∈ M.(accept_states).
-
-Definition accepted_tags (s : Input.t) : ensemble Token.t :=
-  fun tag => accepts s tag.
 
 Lemma delta_star_app (q1 : Q) (q2 : Q) (q3 : Q) (s1 : Input.t) (s2 : Input.t)
   (H1_delta_star : q2 \in delta_star q1 s1)
@@ -253,6 +291,16 @@ Lemma delta_star_app (q1 : Q) (q2 : Q) (q3 : Q) (s1 : Input.t) (s2 : Input.t)
 Proof.
   induction H1_delta_star as [q | q q1' q2' s STEP REST IH | q q1' q2' c s STEP REST IH]; simpl; eauto with *.
 Qed.
+
+Inductive eclosure (q : Q) : ensemble Q :=
+  | eclosure_refl
+    : q \in eclosure q
+  | eclosure_step q1 q2
+    (STEP : q1 ∈ eps_step q)
+    (REST : q2 \in eclosure q1)
+    : q2 \in eclosure q.
+
+#[local] Hint Constructors eclosure : core.
 
 Lemma eclosure_trans (q1 : Q) (q2 : Q) (q3 : Q)
   (H1_eclosure : q2 \in eclosure q1)
@@ -270,10 +318,42 @@ Proof.
   - induction H_eclosure as [q | q q1' q2' STEP REST IH]; simpl; eauto with *.
 Qed.
 
+Lemma delta_star_elim (q1 : Q) (q3 : Q) (s : Input.t)
+  (H_delta_star : q3 \in delta_star q1 s)
+  : ⟪ DELTA_STAR_NIL : s = [] /\ q3 = q1 ⟫ \/ ⟪ DELTA_STAR_EPS : exists q2, q2 ∈ eps_step q1 /\ q3 \in delta_star q2 s ⟫ \/ ⟪ DELTA_STAR_CHAR : exists c, exists s', exists q2, s = c :: s' /\ q2 ∈ char_step q1 c /\ q3 \in delta_star q2 s' ⟫.
+Proof.
+  unnw; destruct H_delta_star as [ | q1' q2' s' STEP REST | q1' q2' c s' STEP REST]; [left | right; left | right; right]; done!.
+Qed.
+
+Lemma delta_star_stuck (q1 : Q) (q2 : Q) (s : Input.t)
+  (NO_EPS : forall q, ~ (q ∈ eps_step q1))
+  (NO_CHAR : forall c, forall q, ~ (q ∈ char_step q1 c))
+  (H_delta_star : q2 \in delta_star q1 s)
+  : s = [] /\ q2 = q1.
+Proof.
+  inv H_delta_star; ss!.
+Qed.
+
+End DELTA_STAR.
+
+#[global] Arguments delta_star_app {Q} {eps_step} {char_step} q1 q2 q3 s1 s2 _ _.
+#[global] Arguments eclosure_trans {Q} {eps_step} q1 q2 q3 _ _.
+#[global] Arguments delta_star_iff_eclosure {Q} {eps_step} {char_step} q q'.
+#[global] Arguments delta_star_elim {Q} {eps_step} {char_step} q1 q3 s _.
+#[global] Arguments delta_star_stuck {Q} {eps_step} {char_step} q1 q2 s _ _ _.
+
+Section BASICS.
+
+Variable M : TaggedENFA.t.
+
+#[local] Notation Q := M.(state).
+#[local] Notation M_delta_star := (delta_star M.(eps_step) M.(char_step)).
+#[local] Notation M_eclosure := (eclosure M.(eps_step)).
+
 Lemma eclosure_okay (q1 : Q) (q2 : Q)
   (OKAY : TaggedENFA.okay M)
   (IN : q1 ∈ M.(states))
-  (H_eclosure : q2 \in eclosure q1)
+  (H_eclosure : q2 \in M_eclosure q1)
   : q2 ∈ M.(states).
 Proof.
   destruct OKAY as [_ _ ? _]; induction H_eclosure as [q | q q1' q2' STEP REST IH]; simpl; eauto with *.
@@ -282,85 +362,1718 @@ Qed.
 Lemma delta_star_okay (q1 : Q) (q2 : Q) (s : Input.t)
   (OKAY : TaggedENFA.okay M)
   (IN : q1 ∈ M.(states))
-  (H_delta_star : q2 \in delta_star q1 s)
+  (H_delta_star : q2 \in M_delta_star q1 s)
   : q2 ∈ M.(states).
 Proof.
   destruct OKAY as [_ _ ? ?]; induction H_delta_star as [q | q q1' q2' s STEP REST IH | q q1' q2' c s STEP REST IH]; simpl; eauto with *.
 Qed.
 
-Lemma delta_star_elim (q1 : Q) (q3 : Q) (s : Input.t)
-  (H_delta_star : q3 \in delta_star q1 s)
-  : ⟪ DELTA_STAR_NIL : s = [] /\ q3 = q1 ⟫ \/ ⟪ DELTA_STAR_EPS : exists q2, q2 ∈ M.(eps_step) q1 /\ q3 \in delta_star q2 s ⟫ \/ ⟪ DELTA_STAR_CHAR : exists c, exists s', exists q2, s = c :: s' /\ q2 ∈ M.(char_step) q1 c /\ q3 \in delta_star q2 s' ⟫.
-Proof.
-  unnw; destruct H_delta_star as [ | q1' q2' s' STEP REST | q1' q2' c s' STEP REST]; [left | right; left | right; right]; done!.
-Qed.
+Definition accepts (s : Input.t) (tag : Token.t) : Prop :=
+  exists qf, qf \in M_delta_star M.(start_state) s /\ (qf, tag) ∈ M.(accept_states).
 
-Lemma delta_star_stuck (q1 : Q) (q2 : Q) (s : Input.t)
-  (NO_EPS : forall q, q ∈ M.(eps_step) q1 -> False)
-  (NO_CHAR : forall c, forall q, q ∈ M.(char_step) q1 c -> False)
-  (H_delta_star : q2 \in delta_star q1 s)
-  : s = [] /\ q2 = q1.
-Proof.
-  inv H_delta_star; ss!.
-Qed.
+Definition accepted_tags (s : Input.t) : ensemble Token.t :=
+  fun tag => accepts s tag.
 
 End BASICS.
 
-End TaggedENFA.
-
-Module Rule.
+Section Thompson's_construction.
 
 #[projections(primitive)]
-Record t : Set :=
-  mk
-  { index : nat
-  ; token : Token.t
-  ; regex : regex ascii
-  }.
+Record char_edge : Set :=
+  mkCharEdge
+  { char_edge_src : nat
+  ; char_edge_label : ascii
+  ; char_edge_dst : nat
+  } as char_edge.
 
-Definition compile_rule (rule : Rule.t) : ErrM Rule.t :=
-  if nullable rule.(regex) then
-    inl (Error.NullableTokenRule rule.(index))
-  else
-    pure rule.
+#[projections(primitive)]
+Record fragment : Set :=
+  mkFragment
+  { frag_start : nat
+  ; frag_accept : nat
+  ; frag_eps_edges : list (nat * nat)
+  ; frag_char_edges : list char_edge
+  } as frag.
 
-Theorem compile_rule_spec (rule : Rule.t) (compiled_rule : Rule.t)
-  (COMPILE : compile_rule rule = inr compiled_rule)
-  : forall s, s \in eval_regex rule.(regex) <-> s \in eval_regex compiled_rule.(regex).
-Proof.
-  intros s; split; intros ACCEPTS; unfold compile_rule in COMPILE; now destruct (nullable rule.(regex)) eqn: NULLABLE; inv COMPILE.
-Qed.
-
-Lemma compile_rule_not_match_empty (rule : Rule.t) (compiled_rule : Rule.t)
-  (COMPILE : compile_rule rule = inr compiled_rule)
-  : ~ [] \in eval_regex compiled_rule.(regex).
-Proof.
-  unfold compile_rule in COMPILE; destruct (nullable rule.(regex)) eqn: NULLABLE; inv COMPILE; now rewrite <- nullable_false_iff.
-Qed.
-
-Lemma possible_output_of_compile_rule (rule : Rule.t) (RET : ErrM Rule.t)
-  (H_RET : compile_rule rule = RET)
-  : match RET with
-    | inl (Error.NoMatch rest) => False
-    | inl Error.InternalInvariantBroken => False
-    | _ => True
-    end.
-Proof.
-  subst RET; unfold compile_rule; destruct (nullable rule.(regex)); simpl; eauto.
-Qed.
-
-Fixpoint compile_rules (rules : list Rule.t) {struct rules} : ErrM (list Rule.t) :=
-  match rules with
-  | [] => pure (@nil Rule.t)
-  | rule :: rules => liftM2 (@cons Rule.t) (compile_rule rule) (compile_rules rules)
+Fixpoint regex2fragment (e : regex ascii) (qi : nat) {struct e} : nat * fragment :=
+  match e with
+  | Re.Null =>
+    let qf := qi + 1 in
+    (qf, mkFragment qi qf [] [])
+  | Re.Empty =>
+    let qf := qi + 1 in
+    (qf, mkFragment qi qf [(qi, qf)] [])
+  | Re.Char c =>
+    let qf := qi + 1 in
+    (qf, mkFragment qi qf [] [mkCharEdge qi c qf])
+  | Re.Union e1 e2 =>
+    let qi1 := qi + 1 in
+    let '(qf1, frag1) := regex2fragment e1 qi1 in
+    let qi2 := qf1 + 1 in
+    let '(qf2, frag2) := regex2fragment e2 qi2 in
+    let qf := qf2 + 1 in
+    (qf, mkFragment qi qf ((qi, qi1) :: (qi, qi2) :: (qf1, qf) :: (qf2, qf) :: frag1.(frag_eps_edges) ++ frag2.(frag_eps_edges)) (frag1.(frag_char_edges) ++ frag2.(frag_char_edges)))
+  | Re.Append e1 e2 =>
+    let qi1 := qi + 1 in
+    let '(qf1, frag1) := regex2fragment e1 qi1 in
+    let qi2 := qf1 + 1 in
+    let '(qf2, frag2) := regex2fragment e2 qi2 in
+    let qf := qf2 + 1 in
+    (qf, mkFragment qi qf ((qi, qi1) :: (qf1, qi2) :: (qf2, qf) :: frag1.(frag_eps_edges) ++ frag2.(frag_eps_edges)) (frag1.(frag_char_edges) ++ frag2.(frag_char_edges)))
+  | Re.Star e1 =>
+    let qi1 := qi + 1 in
+    let '(qf1, frag1) := regex2fragment e1 qi1 in
+    let qf := qf1 + 1 in
+    (qf, mkFragment qi qf ((qi, qi1) :: (qf1, qi1) :: (qi1, qf) :: frag1.(frag_eps_edges)) frag1.(frag_char_edges))
   end.
 
-Definition raws : list Rule.t :=
-  L.mapi_from 1 (fun index => fun '(token, regex) => Rule.mk index token regex) Token.rules.
+Fixpoint rules2fragments (qi : nat) (rules : list Rule.t) {struct rules} : nat * list (Rule.t * fragment) :=
+  match rules with
+  | [] => (qi, [])
+  | rule :: rules' =>
+    let '(qf, frag) := regex2fragment rule.(Rule.regex) qi in
+    let '(qmax, frags) := rules2fragments (qf + 1) rules' in
+    (qmax, (rule, frag) :: frags)
+  end.
 
-Definition compileds : ErrM (list Rule.t) :=
-  compile_rules raws.
+Fixpoint eps_step_from_edges (q : nat) (edges : list (nat * nat)) {struct edges} : list nat :=
+  match edges with
+  | [] => []
+  | (src, dst) :: edges' =>
+    if eq_dec q src then
+      dst :: eps_step_from_edges q edges'
+    else
+      eps_step_from_edges q edges'
+  end.
 
-End Rule.
+Fixpoint char_step_from_edges (q : nat) (c : ascii) (edges : list char_edge) {struct edges} : list nat :=
+  match edges with
+  | [] => []
+  | edge :: edges' =>
+    if eq_dec q edge.(char_edge_src) then
+      if eq_dec c edge.(char_edge_label) then
+        edge.(char_edge_dst) :: char_step_from_edges q c edges'
+      else
+        char_step_from_edges q c edges'
+    else
+      char_step_from_edges q c edges'
+  end.
+
+Fixpoint fragment_eps_edges (frags : list (Rule.t * fragment)) {struct frags} : list (nat * nat) :=
+  match frags with
+  | [] => []
+  | (_, frag) :: frags' => (0, frag.(frag_start)) :: frag.(frag_eps_edges) ++ fragment_eps_edges frags'
+  end.
+
+Fixpoint fragment_char_edges (frags : list (Rule.t * fragment)) {struct frags} : list char_edge :=
+  match frags with
+  | [] => []
+  | (_, frag) :: frags' => frag.(frag_char_edges) ++ fragment_char_edges frags'
+  end.
+
+Definition fragment_accept_states (frags : list (Rule.t * fragment)) : list (nat * Token.t) :=
+  map (fun '(rule, frag) => (frag.(frag_accept), rule.(Rule.token))) frags.
+
+Definition fragments2TaggedENFA (qmax : nat) (frags : list (Rule.t * fragment)) : TaggedENFA.t :=
+  let eps_edges := fragment_eps_edges frags in
+  let char_edges := fragment_char_edges frags in
+  {|
+    state := nat;
+    state_hasEqDec := nat_hasEqDec;
+    states := seq 0 qmax;
+    start_state := 0;
+    accept_states := fragment_accept_states frags;
+    eps_step := fun q => eps_step_from_edges q eps_edges;
+    char_step := fun q => fun c => char_step_from_edges q c char_edges;
+  |}.
+
+Definition mkUnitedTaggedENFA (rules : list Rule.t) : TaggedENFA.t :=
+  let '(qmax, frags) := rules2fragments 1 rules in
+  fragments2TaggedENFA qmax frags.
+
+Lemma eps_step_from_edges_complete (q : nat) (q' : nat) (edges : list (nat * nat))
+  (IN : (q, q') ∈ edges)
+  : q' ∈ eps_step_from_edges q edges.
+Proof.
+  induction edges as [ | [src dst] edges IH]; simpl in IN |- *.
+  - contradiction.
+  - destruct IN as [EQ | IN].
+    + inv EQ. destruct (eq_dec q q) as [_ | NE]; [left; reflexivity | contradiction NE; reflexivity].
+    + destruct (eq_dec q src) as [_ | _]; simpl; eauto.
+Qed.
+
+Lemma eps_step_from_edges_sound (q : nat) (q' : nat) (edges : list (nat * nat))
+  (IN : q' ∈ eps_step_from_edges q edges)
+  : (q, q') ∈ edges.
+Proof.
+  induction edges as [ | [src dst] edges IH]; simpl in IN |- *; ss!.
+  destruct (eq_dec q src) as [EQ | NE]; simpl in IN; done!.
+Qed.
+
+Lemma char_step_from_edges_complete (edge : char_edge) (edges : list char_edge)
+  (IN : edge ∈ edges)
+  : edge.(char_edge_dst) ∈ char_step_from_edges edge.(char_edge_src) edge.(char_edge_label) edges.
+Proof.
+  induction edges as [ | edge' edges IH]; simpl in IN |- *.
+  - contradiction.
+  - destruct IN as [EQ | IN].
+    + subst edge'. destruct (eq_dec edge.(char_edge_src) edge.(char_edge_src)) as [_ | NE]; [ | contradiction NE; reflexivity].
+      destruct (eq_dec edge.(char_edge_label) edge.(char_edge_label)) as [_ | NE]; [left; reflexivity | contradiction NE; reflexivity].
+    + destruct (eq_dec edge.(char_edge_src) edge'.(char_edge_src)) as [_ | _]; destruct (eq_dec edge.(char_edge_label) edge'.(char_edge_label)) as [_ | _]; simpl; eauto.
+Qed.
+
+Lemma char_step_from_edges_sound (q : nat) (q' : nat) (c : ascii) (edges : list char_edge)
+  (IN : q' ∈ char_step_from_edges q c edges)
+  : exists edge, edge ∈ edges /\ edge.(char_edge_src) = q /\ edge.(char_edge_label) = c /\ edge.(char_edge_dst) = q'.
+Proof.
+  induction edges as [ | edge edges IH]; simpl in IN |- *; try tauto.
+  destruct (eq_dec q edge.(char_edge_src)) as [SRC | SRC_NE].
+  - destruct (eq_dec c edge.(char_edge_label)) as [LABEL | LABEL_NE]; simpl in IN.
+    + destruct IN as [DST | IN].
+      * exists edge. subst q'. repeat split; eauto.
+      * pose proof (IH IN) as (edge' & IN_EDGE & SRC' & LABEL' & DST').
+        exists edge'. repeat split; eauto.
+    + pose proof (IH IN) as (edge' & IN_EDGE & SRC' & LABEL' & DST').
+      exists edge'. repeat split; eauto.
+  - pose proof (IH IN) as (edge' & IN_EDGE & SRC' & LABEL' & DST').
+    exists edge'. repeat split; eauto.
+Qed.
+
+Lemma fragment_eps_edges_start_complete (frags : list (Rule.t * fragment)) (rule : Rule.t) (frag : fragment)
+  (IN : (rule, frag) ∈ frags)
+  : (0, frag.(frag_start)) ∈ fragment_eps_edges frags.
+Proof.
+  induction frags as [ | [rule' frag'] frags IH]; simpl in IN |- *; eauto.
+  destruct IN as [EQ | IN]; [inv EQ; left; reflexivity | right; rewrite in_app_iff; right; eauto].
+Qed.
+
+Lemma fragment_eps_edges_complete (frags : list (Rule.t * fragment)) (rule : Rule.t) (frag : fragment) (q : nat) (q' : nat)
+  (IN_FRAG : (rule, frag) ∈ frags)
+  (IN_EDGE : (q, q') ∈ frag.(frag_eps_edges))
+  : (q, q') ∈ fragment_eps_edges frags.
+Proof.
+  induction frags as [ | [rule' frag'] frags IH]; simpl in IN_FRAG |- *; eauto.
+  destruct IN_FRAG as [EQ | IN_FRAG].
+  - inv EQ. right. rewrite in_app_iff. left. exact IN_EDGE.
+  - right. rewrite in_app_iff. right. eauto.
+Qed.
+
+Lemma fragment_char_edges_complete (frags : list (Rule.t * fragment)) (rule : Rule.t) (frag : fragment) (edge : char_edge)
+  (IN_FRAG : (rule, frag) ∈ frags)
+  (IN_EDGE : edge ∈ frag.(frag_char_edges))
+  : edge ∈ fragment_char_edges frags.
+Proof.
+  induction frags as [ | [rule' frag'] frags IH]; simpl in IN_FRAG |- *; eauto.
+  destruct IN_FRAG as [EQ | IN_FRAG].
+  - inv EQ. rewrite in_app_iff. left. exact IN_EDGE.
+  - rewrite in_app_iff. right. eauto.
+Qed.
+
+Lemma fragment_accept_states_complete (frags : list (Rule.t * fragment)) (rule : Rule.t) (frag : fragment)
+  (IN_FRAG : (rule, frag) ∈ frags)
+  : (frag.(frag_accept), rule.(Rule.token)) ∈ fragment_accept_states frags.
+Proof.
+  unfold fragment_accept_states. rewrite L.in_map_iff.
+  exists (rule, frag). split; [reflexivity | exact IN_FRAG].
+Qed.
+
+Lemma fragment_accept_states_sound (frags : list (Rule.t * fragment)) q tag
+  (IN : (q, tag) ∈ fragment_accept_states frags)
+  : exists rule, exists frag, (rule, frag) ∈ frags /\ q = frag.(frag_accept) /\ tag = rule.(Rule.token).
+Proof.
+  unfold fragment_accept_states in IN. rewrite L.in_map_iff in IN.
+  destruct IN as ([rule frag] & EQ & IN_FRAG). inv EQ.
+  exists rule, frag. eauto.
+Qed.
+
+Variant TaggedENFA_COMPILED (M : TaggedENFA.t) rules qmax frags : Prop :=
+  | TaggedENFA_COMPILED_intro 
+    (COMPILED_RULES : Rule.compileds = inr rules)
+    (COMPILED_ENFA : M = mkUnitedTaggedENFA rules)
+    (COMPILED_FRAGS : rules2fragments 1 rules = (qmax, frags)).
+
+Variant TaggedENFA_FRAGMENTS (frags : list (Rule.t * fragment)) rule frag : Prop :=
+  | TaggedENFA_FRAGMENTS_intro
+    (IN1 : frag.(frag_start) ∈ eps_step_from_edges 0 (fragment_eps_edges frags))
+    (IN2 : (frag.(frag_accept), rule.(Rule.token)) ∈ fragment_accept_states frags)
+    (EPS : forall q, forall q', (q, q') ∈ frag.(frag_eps_edges) -> q' ∈ eps_step_from_edges q (fragment_eps_edges frags))
+    (CHAR : forall edge, edge ∈ frag.(frag_char_edges) -> edge.(char_edge_dst) ∈ char_step_from_edges edge.(char_edge_src) edge.(char_edge_label) (fragment_char_edges frags)).
+
+Theorem mkUnitedTaggedENFA_spec (M : TaggedENFA.t)
+  (COMPILE : fmap mkUnitedTaggedENFA Rule.compileds = inr M)
+  : exists rules, exists qmax, exists frags, TaggedENFA_COMPILED M rules qmax frags /\ (forall rule, forall frag, (rule, frag) ∈ frags -> TaggedENFA_FRAGMENTS frags rule frag).
+Proof.
+  unfold fmap, mkFunctorFromMonad in COMPILE. simpl in COMPILE.
+  destruct Rule.compileds as [err | rules] eqn: COMPILED; inv COMPILE.
+  destruct (rules2fragments 1 rules) as [qmax frags] eqn: FRAGS.
+  exists rules, qmax, frags. split.
+  - econs; eauto.
+  - ii; econs.
+    + eapply eps_step_from_edges_complete. eapply fragment_eps_edges_start_complete. exact H.
+    + eapply fragment_accept_states_complete. exact H.
+    + intros q q' IN_EDGE. eapply eps_step_from_edges_complete. eapply fragment_eps_edges_complete; eauto.
+    + intros edge IN_EDGE. eapply char_step_from_edges_complete. eapply fragment_char_edges_complete; eauto.
+Qed.
+
+Definition fragments_delta_star (frags : list (Rule.t * fragment)) : nat -> Input.t -> ensemble nat :=
+  delta_star (fun q => eps_step_from_edges q (fragment_eps_edges frags)) (fun q c => char_step_from_edges q c (fragment_char_edges frags)).
+
+Definition fragment_delta_star (frag : fragment) : nat -> Input.t -> ensemble nat :=
+  delta_star (fun q => eps_step_from_edges q frag.(frag_eps_edges)) (fun q c => char_step_from_edges q c frag.(frag_char_edges)).
+
+Lemma mkUnitedTaggedENFA_unfold_fragments rules qmax frags
+  (FRAGS : rules2fragments 1 rules = (qmax, frags))
+  : mkUnitedTaggedENFA rules = fragments2TaggedENFA qmax frags.
+Proof.
+  unfold mkUnitedTaggedENFA, fragments2TaggedENFA. rewrite FRAGS. reflexivity.
+Qed.
+
+Lemma TaggedENFA_COMPILED_as_fragments M rules qmax frags
+  (COMPILED : TaggedENFA_COMPILED M rules qmax frags)
+  : M = fragments2TaggedENFA qmax frags.
+Proof.
+  inv COMPILED. eapply mkUnitedTaggedENFA_unfold_fragments. exact COMPILED_FRAGS.
+Qed.
+
+Lemma TaggedENFA_FRAGMENTS_delta_star_step frags rule frag
+  (FRAGMENTS : TaggedENFA_FRAGMENTS frags rule frag)
+  : ⟪ EPS : forall q, forall q', (q, q') ∈ frag.(frag_eps_edges) -> q' \in fragments_delta_star frags q [] ⟫ /\ ⟪ CHAR : forall edge, edge ∈ frag.(frag_char_edges) -> edge.(char_edge_dst) \in fragments_delta_star frags edge.(char_edge_src) [edge.(char_edge_label)] ⟫.
+Proof.
+  destruct FRAGMENTS as [_ _ EPS CHAR]. split.
+  - intros q q' IN_EDGE. eapply delta_star_eps with (q1 := q').
+    + exact (EPS q q' IN_EDGE).
+    + econs.
+  - intros edge IN_EDGE. eapply delta_star_char with (q1 := edge.(char_edge_dst)).
+    + exact (CHAR edge IN_EDGE).
+    + econs.
+Qed.
+
+Lemma regex2fragment_empty_delta_star frags rule qi qf frag
+  (REGEX2FRAGMENT : regex2fragment Re.Empty qi = (qf, frag))
+  (FRAGMENTS : TaggedENFA_FRAGMENTS frags rule frag)
+  : frag.(frag_accept) \in fragments_delta_star frags frag.(frag_start) [].
+Proof.
+  pose proof (TaggedENFA_FRAGMENTS_delta_star_step frags rule frag FRAGMENTS) as [EPS _].
+  simpl in REGEX2FRAGMENT. inv REGEX2FRAGMENT. eapply EPS. simpl. left. reflexivity.
+Qed.
+
+Lemma regex2fragment_start_accept e qi qf frag
+  (REGEX2FRAGMENT : regex2fragment e qi = (qf, frag))
+  : frag.(frag_start) = qi /\ frag.(frag_accept) = qf.
+Proof.
+  revert qi qf frag REGEX2FRAGMENT.
+  induction e as [ | | c | e1 IH1 e2 IH2 | e1 IH1 e2 IH2 | e IH]; intros qi qf frag REGEX2FRAGMENT; simpl in REGEX2FRAGMENT.
+  - inv REGEX2FRAGMENT. eauto.
+  - inv REGEX2FRAGMENT. eauto.
+  - inv REGEX2FRAGMENT. eauto.
+  - destruct (regex2fragment e1 (qi + 1)) as [qf1 frag1].
+    destruct (regex2fragment e2 (qf1 + 1)) as [qf2 frag2].
+    inv REGEX2FRAGMENT. eauto.
+  - destruct (regex2fragment e1 (qi + 1)) as [qf1 frag1].
+    destruct (regex2fragment e2 (qf1 + 1)) as [qf2 frag2].
+    inv REGEX2FRAGMENT. eauto.
+  - destruct (regex2fragment e (qi + 1)) as [qf1 frag1].
+    inv REGEX2FRAGMENT. eauto.
+Qed.
+
+Lemma regex2fragment_same_fragment e qi1 qf1 qi2 qf2 frag
+  (REGEX1 : regex2fragment e qi1 = (qf1, frag))
+  (REGEX2 : regex2fragment e qi2 = (qf2, frag))
+  : qi1 = qi2 /\ qf1 = qf2.
+Proof.
+  pose proof (regex2fragment_start_accept _ _ _ _ REGEX1) as [START1 ACCEPT1].
+  pose proof (regex2fragment_start_accept _ _ _ _ REGEX2) as [START2 ACCEPT2].
+  split; congruence.
+Qed.
+
+Definition eps_edge_in_range (lo : nat) (hi : nat) (edge : nat * nat) : Prop :=
+  lo <= fst edge <= hi /\ lo <= snd edge <= hi.
+
+Definition char_edge_in_range (lo : nat) (hi : nat) (edge : char_edge) : Prop :=
+  lo <= edge.(char_edge_src) <= hi /\ lo <= edge.(char_edge_dst) <= hi.
+
+Variant FRAGMENT_BOUNDS (lo : nat) (hi : nat) (frag : fragment) : Prop :=
+  | FRAGMENT_BOUNDS_intro
+    (BOUNDS_START : frag.(frag_start) = lo)
+    (BOUNDS_ACCEPT : frag.(frag_accept) = hi)
+    (BOUNDS_LT : lo < hi)
+    (BOUNDS_EPS : forall edge, edge ∈ frag.(frag_eps_edges) -> eps_edge_in_range lo hi edge)
+    (BOUNDS_CHAR : forall edge, edge ∈ frag.(frag_char_edges) -> char_edge_in_range lo hi edge).
+
+Lemma regex2fragment_bounds e qi qf frag
+  (REGEX2FRAGMENT : regex2fragment e qi = (qf, frag))
+  : FRAGMENT_BOUNDS qi qf frag.
+Proof.
+  revert qi qf frag REGEX2FRAGMENT.
+  induction e as [ | | c | e1 IH1 e2 IH2 | e1 IH1 e2 IH2 | e IH]; intros qi qf frag REGEX2FRAGMENT; simpl in REGEX2FRAGMENT.
+  - inv REGEX2FRAGMENT. econs; simpl; try lia; tauto.
+  - inv REGEX2FRAGMENT. econs; simpl; try lia.
+    intros [q q'] [EQ | IN].
+    + injection EQ as EQ1 EQ2. subst. unfold eps_edge_in_range. simpl. lia.
+    + contradiction.
+  - inv REGEX2FRAGMENT. econs; simpl; try lia.
+    intros edge [EQ | IN]; [subst edge; unfold char_edge_in_range; simpl; lia | contradiction].
+  - destruct (regex2fragment e1 (qi + 1)) as [qf1 frag1] eqn: REGEX1.
+    destruct (regex2fragment e2 (qf1 + 1)) as [qf2 frag2] eqn: REGEX2.
+    pose proof (IH1 _ _ _ REGEX1) as [START1 ACCEPT1 LT1 EPS1 CHAR1].
+    pose proof (IH2 _ _ _ REGEX2) as [START2 ACCEPT2 LT2 EPS2 CHAR2].
+    inv REGEX2FRAGMENT. econs; simpl; try lia.
+    + intros [q q'] IN_EDGE. simpl in IN_EDGE.
+      destruct IN_EDGE as [EQ | [EQ | [EQ | [EQ | IN_EDGE]]]].
+      * injection EQ as EQ1 EQ2. subst. unfold eps_edge_in_range. simpl. lia.
+      * injection EQ as EQ1 EQ2. subst. unfold eps_edge_in_range. simpl. lia.
+      * injection EQ as EQ1 EQ2. subst. unfold eps_edge_in_range. simpl. lia.
+      * injection EQ as EQ1 EQ2. subst. unfold eps_edge_in_range. simpl. lia.
+      * rewrite in_app_iff in IN_EDGE. destruct IN_EDGE as [IN_EDGE | IN_EDGE].
+        { pose proof (EPS1 _ IN_EDGE). unfold eps_edge_in_range in *. simpl in *. lia. }
+        { pose proof (EPS2 _ IN_EDGE). unfold eps_edge_in_range in *. simpl in *. lia. }
+    + intros edge IN_EDGE. simpl in IN_EDGE. rewrite in_app_iff in IN_EDGE.
+      destruct IN_EDGE as [IN_EDGE | IN_EDGE].
+      * pose proof (CHAR1 _ IN_EDGE). unfold char_edge_in_range in *. lia.
+      * pose proof (CHAR2 _ IN_EDGE). unfold char_edge_in_range in *. lia.
+  - destruct (regex2fragment e1 (qi + 1)) as [qf1 frag1] eqn: REGEX1.
+    destruct (regex2fragment e2 (qf1 + 1)) as [qf2 frag2] eqn: REGEX2.
+    pose proof (IH1 _ _ _ REGEX1) as [START1 ACCEPT1 LT1 EPS1 CHAR1].
+    pose proof (IH2 _ _ _ REGEX2) as [START2 ACCEPT2 LT2 EPS2 CHAR2].
+    inv REGEX2FRAGMENT. econs; simpl; try lia.
+    + intros [q q'] IN_EDGE. simpl in IN_EDGE.
+      destruct IN_EDGE as [EQ | [EQ | [EQ | IN_EDGE]]].
+      * injection EQ as EQ1 EQ2. subst. unfold eps_edge_in_range. simpl. lia.
+      * injection EQ as EQ1 EQ2. subst. unfold eps_edge_in_range. simpl. lia.
+      * injection EQ as EQ1 EQ2. subst. unfold eps_edge_in_range. simpl. lia.
+      * rewrite in_app_iff in IN_EDGE. destruct IN_EDGE as [IN_EDGE | IN_EDGE].
+        { pose proof (EPS1 _ IN_EDGE). unfold eps_edge_in_range in *. simpl in *. lia. }
+        { pose proof (EPS2 _ IN_EDGE). unfold eps_edge_in_range in *. simpl in *. lia. }
+    + intros edge IN_EDGE. simpl in IN_EDGE. rewrite in_app_iff in IN_EDGE.
+      destruct IN_EDGE as [IN_EDGE | IN_EDGE].
+      * pose proof (CHAR1 _ IN_EDGE). unfold char_edge_in_range in *. lia.
+      * pose proof (CHAR2 _ IN_EDGE). unfold char_edge_in_range in *. lia.
+  - destruct (regex2fragment e (qi + 1)) as [qf1 frag1] eqn: REGEX1.
+    pose proof (IH _ _ _ REGEX1) as [START1 ACCEPT1 LT1 EPS1 CHAR1].
+    inv REGEX2FRAGMENT. econs; simpl; try lia.
+    + intros [q q'] IN_EDGE. simpl in IN_EDGE.
+      destruct IN_EDGE as [EQ | [EQ | [EQ | IN_EDGE]]].
+      * injection EQ as EQ1 EQ2. subst. unfold eps_edge_in_range. simpl. lia.
+      * injection EQ as EQ1 EQ2. subst. unfold eps_edge_in_range. simpl. lia.
+      * injection EQ as EQ1 EQ2. subst. unfold eps_edge_in_range. simpl. lia.
+      * pose proof (EPS1 _ IN_EDGE). unfold eps_edge_in_range in *. simpl in *. lia.
+    + intros edge IN_EDGE.
+      pose proof (CHAR1 _ IN_EDGE). unfold char_edge_in_range in *. lia.
+Qed.
+
+Lemma regex2fragment_edge_src_lt e qi qf frag
+  (REGEX2FRAGMENT : regex2fragment e qi = (qf, frag))
+  : (forall q, forall q', (q, q') ∈ frag.(frag_eps_edges) -> q < qf) /\ (forall edge, edge ∈ frag.(frag_char_edges) -> edge.(char_edge_src) < qf).
+Proof.
+  revert qi qf frag REGEX2FRAGMENT.
+  induction e as [ | | c | e1 IH1 e2 IH2 | e1 IH1 e2 IH2 | e IH]; ii; simpl in REGEX2FRAGMENT.
+  - inv REGEX2FRAGMENT. split; ii; contradiction.
+  - inv REGEX2FRAGMENT. split; ii; simpl in *.
+    + destruct H as [EQ | []]. inv EQ. lia.
+    + contradiction.
+  - inv REGEX2FRAGMENT. split; ii; simpl in *.
+    + contradiction.
+    + destruct H as [EQ | []]. subst edge. simpl. lia.
+  - destruct (regex2fragment e1 (qi + 1)) as [qf1 frag1] eqn: REGEX1.
+    destruct (regex2fragment e2 (qf1 + 1)) as [qf2 frag2] eqn: REGEX2.
+    pose proof (IH1 _ _ _ REGEX1) as [EPS1 CHAR1].
+    pose proof (IH2 _ _ _ REGEX2) as [EPS2 CHAR2].
+    pose proof (regex2fragment_bounds _ _ _ _ REGEX1) as [_ _ LT1 _ _].
+    pose proof (regex2fragment_bounds _ _ _ _ REGEX2) as [_ _ LT2 _ _].
+    inv REGEX2FRAGMENT. split; ii; simpl in *.
+    + des; try (inv H; lia). rewrite in_app_iff in H. des; eauto; [pose proof (EPS1 _ _ H) | pose proof (EPS2 _ _ H)]; lia.
+    + rewrite in_app_iff in H. des; eauto; [pose proof (CHAR1 _ H) | pose proof (CHAR2 _ H)]; lia.
+  - destruct (regex2fragment e1 (qi + 1)) as [qf1 frag1] eqn: REGEX1.
+    destruct (regex2fragment e2 (qf1 + 1)) as [qf2 frag2] eqn: REGEX2.
+    pose proof (IH1 _ _ _ REGEX1) as [EPS1 CHAR1].
+    pose proof (IH2 _ _ _ REGEX2) as [EPS2 CHAR2].
+    pose proof (regex2fragment_bounds _ _ _ _ REGEX1) as [_ _ LT1 _ _].
+    pose proof (regex2fragment_bounds _ _ _ _ REGEX2) as [_ _ LT2 _ _].
+    inv REGEX2FRAGMENT. split; ii; simpl in *.
+    + des; try (inv H; lia). rewrite in_app_iff in H. des; eauto; [pose proof (EPS1 _ _ H) | pose proof (EPS2 _ _ H)]; lia.
+    + rewrite in_app_iff in H. des; eauto; [pose proof (CHAR1 _ H) | pose proof (CHAR2 _ H)]; lia.
+  - destruct (regex2fragment e (qi + 1)) as [qf1 frag1] eqn: REGEX.
+    pose proof (IH _ _ _ REGEX) as [EPS1 CHAR1].
+    pose proof (regex2fragment_bounds _ _ _ _ REGEX) as [_ _ LT1 _ _].
+    inv REGEX2FRAGMENT. split; ii; simpl in *.
+    + des; try (inv H; lia). pose proof (EPS1 _ _ H). lia.
+    + pose proof (CHAR1 _ H). lia.
+Qed.
+
+Lemma regex2fragment_edge_dst_gt_start e qi qf frag
+  (REGEX2FRAGMENT : regex2fragment e qi = (qf, frag))
+  : (forall q, forall q', (q, q') ∈ frag.(frag_eps_edges) -> qi < q') /\ (forall edge, edge ∈ frag.(frag_char_edges) -> qi < edge.(char_edge_dst)).
+Proof.
+  revert qi qf frag REGEX2FRAGMENT.
+  induction e as [ | | c | e1 IH1 e2 IH2 | e1 IH1 e2 IH2 | e IH]; ii; simpl in REGEX2FRAGMENT.
+  - inv REGEX2FRAGMENT. split; ii; contradiction.
+  - inv REGEX2FRAGMENT. split; ii; simpl in *.
+    + destruct H as [EQ | []]. inv EQ. lia.
+    + contradiction.
+  - inv REGEX2FRAGMENT. split; ii; simpl in *.
+    + contradiction.
+    + destruct H as [EQ | []]. subst edge. simpl. lia.
+  - destruct (regex2fragment e1 (qi + 1)) as [qf1 frag1] eqn: REGEX1.
+    destruct (regex2fragment e2 (qf1 + 1)) as [qf2 frag2] eqn: REGEX2.
+    pose proof (IH1 _ _ _ REGEX1) as [EPS1 CHAR1].
+    pose proof (IH2 _ _ _ REGEX2) as [EPS2 CHAR2].
+    pose proof (regex2fragment_bounds _ _ _ _ REGEX1) as [_ _ LT1 _ _].
+    pose proof (regex2fragment_bounds _ _ _ _ REGEX2) as [_ _ LT2 _ _].
+    inv REGEX2FRAGMENT. split; ii; simpl in *.
+    + des; try (inv H; lia). rewrite in_app_iff in H. des; [pose proof (EPS1 _ _ H) | pose proof (EPS2 _ _ H)]; lia.
+    + rewrite in_app_iff in H. des; [pose proof (CHAR1 _ H) | pose proof (CHAR2 _ H)]; lia.
+  - destruct (regex2fragment e1 (qi + 1)) as [qf1 frag1] eqn: REGEX1.
+    destruct (regex2fragment e2 (qf1 + 1)) as [qf2 frag2] eqn: REGEX2.
+    pose proof (IH1 _ _ _ REGEX1) as [EPS1 CHAR1].
+    pose proof (IH2 _ _ _ REGEX2) as [EPS2 CHAR2].
+    pose proof (regex2fragment_bounds _ _ _ _ REGEX1) as [_ _ LT1 _ _].
+    pose proof (regex2fragment_bounds _ _ _ _ REGEX2) as [_ _ LT2 _ _].
+    inv REGEX2FRAGMENT. split; ii; simpl in *.
+    + des; try (inv H; lia). rewrite in_app_iff in H. des; [pose proof (EPS1 _ _ H) | pose proof (EPS2 _ _ H)]; lia.
+    + rewrite in_app_iff in H. des; [pose proof (CHAR1 _ H) | pose proof (CHAR2 _ H)]; lia.
+  - destruct (regex2fragment e (qi + 1)) as [qf1 frag1] eqn: REGEX.
+    pose proof (IH _ _ _ REGEX) as [EPS1 CHAR1].
+    pose proof (regex2fragment_bounds _ _ _ _ REGEX) as [_ _ LT1 _ _].
+    inv REGEX2FRAGMENT. split; ii; simpl in *.
+    + des; try (inv H; lia). pose proof (EPS1 _ _ H). lia.
+    + pose proof (CHAR1 _ H). lia.
+Qed.
+
+Lemma regex2fragment_complete_aux (e : regex ascii) (s : Input.t) (frags : list (Rule.t * fragment)) (rule : Rule.t) (qi : nat) (qf : nat) (frag topfrag : fragment)
+  (IN_REGEX : s \in eval_regex e)
+  (REGEX2FRAGMENT : regex2fragment e qi = (qf, frag))
+  (FRAGMENTS : TaggedENFA_FRAGMENTS frags rule topfrag)
+  (EPS_INCL : forall q, forall q', (q, q') ∈ frag.(frag_eps_edges) -> (q, q') ∈ topfrag.(frag_eps_edges))
+  (CHAR_INCL : forall edge, edge ∈ frag.(frag_char_edges) -> edge ∈ topfrag.(frag_char_edges))
+  : frag.(frag_accept) \in fragments_delta_star frags frag.(frag_start) s.
+Proof.
+  revert s IN_REGEX frags rule qi qf frag topfrag REGEX2FRAGMENT FRAGMENTS EPS_INCL CHAR_INCL.
+  induction e as [ | | c | e1 IH1 e2 IH2 | e1 IH1 e2 IH2 | e IH]; ii.
+  - simpl in IN_REGEX. contradiction.
+  - simpl in IN_REGEX. autorewrite with simplication_hints in IN_REGEX.
+    subst s. simpl in REGEX2FRAGMENT. inv REGEX2FRAGMENT.
+    pose proof (TaggedENFA_FRAGMENTS_delta_star_step frags rule topfrag FRAGMENTS) as [EPS _].
+    eapply EPS. eapply EPS_INCL. simpl. left. reflexivity.
+  - simpl in IN_REGEX. autorewrite with simplication_hints in IN_REGEX.
+    subst s. simpl in REGEX2FRAGMENT. inv REGEX2FRAGMENT.
+    pose proof (TaggedENFA_FRAGMENTS_delta_star_step frags rule topfrag FRAGMENTS) as [_ CHAR].
+    eapply (CHAR (mkCharEdge qi c (qi + 1))).
+    eapply CHAR_INCL. simpl. left. reflexivity.
+  - simpl in REGEX2FRAGMENT. cbn [eval_regex] in IN_REGEX.
+    autorewrite with simplication_hints in IN_REGEX.
+    destruct (regex2fragment e1 (qi + 1)) as [qf1 frag1] eqn: REGEX1.
+    destruct (regex2fragment e2 (qf1 + 1)) as [qf2 frag2] eqn: REGEX2.
+    inv REGEX2FRAGMENT. destruct IN_REGEX as [IN1 | IN2].
+    + pose proof (TaggedENFA_FRAGMENTS_delta_star_step frags rule topfrag FRAGMENTS) as [EPS _].
+      pose proof (regex2fragment_start_accept _ _ _ _ REGEX1) as [START1 ACCEPT1].
+      rewrite <- app_nil_r with (l := s).
+      eapply delta_star_app with (q2 := qf1).
+      * change s with ([] ++ s).
+        eapply delta_star_app with (q2 := qi + 1).
+        { eapply EPS. eapply EPS_INCL. simpl. left. reflexivity. }
+        { rewrite <- START1. rewrite <- ACCEPT1.
+          eapply (IH1 s IN1 frags rule (qi + 1) qf1 frag1 topfrag REGEX1 FRAGMENTS).
+          - intros q q' IN_EDGE. eapply EPS_INCL. simpl.
+            right; right; right; right. rewrite in_app_iff. left. exact IN_EDGE.
+          - intros edge IN_EDGE. eapply CHAR_INCL. simpl.
+            rewrite in_app_iff. left. exact IN_EDGE.
+        }
+      * eapply EPS. eapply EPS_INCL. simpl. right; right; left. reflexivity.
+    + pose proof (TaggedENFA_FRAGMENTS_delta_star_step frags rule topfrag FRAGMENTS) as [EPS _].
+      pose proof (regex2fragment_start_accept _ _ _ _ REGEX2) as [START2 ACCEPT2].
+      rewrite <- app_nil_r with (l := s).
+      eapply delta_star_app with (q2 := qf2).
+      * change s with ([] ++ s).
+        eapply delta_star_app with (q2 := qf1 + 1).
+        { eapply EPS. eapply EPS_INCL. simpl. right; left. reflexivity. }
+        { rewrite <- START2. rewrite <- ACCEPT2.
+          eapply (IH2 s IN2 frags rule (qf1 + 1) qf2 frag2 topfrag REGEX2 FRAGMENTS).
+          - intros q q' IN_EDGE. eapply EPS_INCL. simpl.
+            right; right; right; right. rewrite in_app_iff. right. exact IN_EDGE.
+          - intros edge IN_EDGE. eapply CHAR_INCL. simpl.
+            rewrite in_app_iff. right. exact IN_EDGE.
+        }
+      * eapply EPS. eapply EPS_INCL. simpl.
+        right; right; right; left. reflexivity.
+  - simpl in REGEX2FRAGMENT. cbn [eval_regex] in IN_REGEX.
+    rewrite E.liftM2_spec in IN_REGEX.
+    destruct (regex2fragment e1 (qi + 1)) as [qf1 frag1] eqn: REGEX1.
+    destruct (regex2fragment e2 (qf1 + 1)) as [qf2 frag2] eqn: REGEX2.
+    inv REGEX2FRAGMENT.
+    destruct IN_REGEX as (s1 & IN1 & s2 & IN2 & EQ). subst s.
+    pose proof (TaggedENFA_FRAGMENTS_delta_star_step frags rule topfrag FRAGMENTS) as [EPS _].
+    pose proof (regex2fragment_start_accept _ _ _ _ REGEX1) as [START1 ACCEPT1].
+    pose proof (regex2fragment_start_accept _ _ _ _ REGEX2) as [START2 ACCEPT2].
+    eapply delta_star_app with (q2 := qf1) (s1 := s1) (s2 := s2).
+    + change s1 with ([] ++ s1).
+      eapply delta_star_app with (q2 := qi + 1).
+      * eapply EPS. eapply EPS_INCL. simpl. left. reflexivity.
+      * rewrite <- START1. rewrite <- ACCEPT1.
+        eapply (IH1 s1 IN1 frags rule (qi + 1) qf1 frag1 topfrag REGEX1 FRAGMENTS).
+        { intros q q' IN_EDGE. eapply EPS_INCL. simpl.
+          right; right; right. rewrite in_app_iff. left. exact IN_EDGE.
+        }
+        { intros edge IN_EDGE. eapply CHAR_INCL. simpl.
+          rewrite in_app_iff. left. exact IN_EDGE.
+        }
+    + rewrite <- app_nil_r with (l := s2).
+      eapply delta_star_app with (q2 := qf2).
+      * change s2 with ([] ++ s2).
+        eapply delta_star_app with (q2 := qf1 + 1).
+        { eapply EPS. eapply EPS_INCL. simpl. right; left. reflexivity. }
+        { rewrite <- START2. rewrite <- ACCEPT2.
+          eapply (IH2 s2 IN2 frags rule (qf1 + 1) qf2 frag2 topfrag REGEX2 FRAGMENTS).
+          - intros q q' IN_EDGE. eapply EPS_INCL. simpl.
+            right; right; right. rewrite in_app_iff. right. exact IN_EDGE.
+          - intros edge IN_EDGE. eapply CHAR_INCL. simpl.
+            rewrite in_app_iff. right. exact IN_EDGE.
+        }
+      * eapply EPS. eapply EPS_INCL. simpl. right; right; left. reflexivity.
+  - simpl in REGEX2FRAGMENT. simpl in IN_REGEX.
+    destruct (regex2fragment e (qi + 1)) as [qf1 frag1] eqn: REGEX1.
+    inv REGEX2FRAGMENT.
+    pose proof (TaggedENFA_FRAGMENTS_delta_star_step frags rule topfrag FRAGMENTS) as [EPS _].
+    pose proof (regex2fragment_start_accept _ _ _ _ REGEX1) as [START1 ACCEPT1].
+    assert (TAIL : forall t, t \in star (eval_regex e) -> qf1 + 1 \in fragments_delta_star frags (qi + 1) t).
+    { intros t STAR_IN. induction STAR_IN as [ | s1 s2 IN1 IN2 IHSTAR].
+      - eapply EPS. eapply EPS_INCL. simpl. right; right; left. reflexivity.
+      - replace (s1 ++ s2) with ((s1 ++ []) ++ s2) by now rewrite app_nil_r.
+        eapply delta_star_app with (q2 := qi + 1).
+        + eapply delta_star_app with (q2 := qf1).
+          * rewrite <- START1. rewrite <- ACCEPT1.
+            eapply (IH s1 IN1 frags rule (qi + 1) qf1 frag1 topfrag REGEX1 FRAGMENTS).
+            { intros q q' IN_EDGE. eapply EPS_INCL. simpl. right; right; right. exact IN_EDGE. }
+            { intros edge IN_EDGE. eapply CHAR_INCL. simpl. exact IN_EDGE. }
+          * eapply EPS. eapply EPS_INCL. simpl. right; left. reflexivity.
+        + exact IHSTAR.
+    }
+    change s with ([] ++ s).
+    eapply delta_star_app with (q2 := qi + 1).
+    + eapply EPS. eapply EPS_INCL. simpl. left. reflexivity.
+    + eapply TAIL. exact IN_REGEX.
+Qed.
+
+Theorem regex2fragment_complete frags rule qi qf frag s
+  (REGEX2FRAGMENT : regex2fragment rule.(Rule.regex) qi = (qf, frag))
+  (FRAGMENTS : TaggedENFA_FRAGMENTS frags rule frag)
+  (IN_REGEX : s \in eval_regex rule.(Rule.regex))
+  : frag.(frag_accept) \in fragments_delta_star frags frag.(frag_start) s.
+Proof.
+  eapply regex2fragment_complete_aux; eauto.
+Qed.
+
+Theorem TaggedENFA_FRAGMENTS_complete qmax frags rule qi qf frag s
+  (REGEX2FRAGMENT : regex2fragment rule.(Rule.regex) qi = (qf, frag))
+  (FRAGMENTS : TaggedENFA_FRAGMENTS frags rule frag)
+  (IN_REGEX : s \in eval_regex rule.(Rule.regex))
+  : accepts (fragments2TaggedENFA qmax frags) s rule.(Rule.token).
+Proof.
+  destruct FRAGMENTS as [START ACCEPT EPS CHAR].
+  exists frag.(frag_accept). split.
+  - change s with ([] ++ s).
+    eapply delta_star_app with (q2 := frag.(frag_start)).
+    + eapply delta_star_eps with (q1 := frag.(frag_start)).
+      * exact START.
+      * econs.
+    + eapply regex2fragment_complete; eauto.
+      econs; eauto.
+  - exact ACCEPT.
+Qed.
+
+Theorem rules2fragments_complete qi rules qmax frags rule
+  (FRAGS : rules2fragments qi rules = (qmax, frags))
+  (IN_RULE : rule ∈ rules)
+  : exists qi_rule, exists qf, exists frag, regex2fragment rule.(Rule.regex) qi_rule = (qf, frag) /\ (rule, frag) ∈ frags.
+Proof.
+  revert qi qmax frags FRAGS IN_RULE.
+  induction rules as [ | rule' rules IH]; intros qi qmax frags FRAGS IN_RULE; simpl in IN_RULE; try tauto.
+  simpl in FRAGS. destruct (regex2fragment rule'.(Rule.regex) qi) as [qf frag] eqn: REGEX2FRAGMENT.
+  destruct (rules2fragments (qf + 1) rules) as [qmax' frags'] eqn: FRAGS'.
+  injection FRAGS as Hqmax Hfrags. subst qmax frags.
+  destruct IN_RULE as [EQ | IN_RULE].
+  - subst rule'. exists qi, qf, frag. split; [exact REGEX2FRAGMENT | left; reflexivity].
+  - pose proof (IH (qf + 1) qmax' frags' FRAGS' IN_RULE) as (qi_rule & qf_rule & frag_rule & REGEX & IN_FRAGS).
+    exists qi_rule, qf_rule, frag_rule. split; [exact REGEX | right; exact IN_FRAGS].
+Qed.
+
+Lemma rules2fragments_sound qi rules qmax frags rule frag
+  (FRAGS : rules2fragments qi rules = (qmax, frags))
+  (IN_FRAG : (rule, frag) ∈ frags)
+  : rule ∈ rules.
+Proof.
+  revert qi qmax frags FRAGS IN_FRAG.
+  induction rules as [ | rule' rules IH]; ii; simpl in FRAGS.
+  - inv FRAGS. contradiction.
+  - destruct (regex2fragment rule'.(Rule.regex) qi) as [qf frag'] eqn: REGEX.
+    destruct (rules2fragments (qf + 1) rules) as [qmax' frags'] eqn: FRAGS'.
+    injection FRAGS as Hqmax Hfrags. subst qmax frags.
+    simpl in IN_FRAG. destruct IN_FRAG as [EQ | IN_FRAG].
+    + inv EQ. left. reflexivity.
+    + right. eapply IH; eauto.
+Qed.
+
+Lemma rules2fragments_bounds qi rules qmax frags
+  (FRAGS : rules2fragments qi rules = (qmax, frags))
+  : qi <= qmax /\ ⟪ BOUND : forall rule, forall frag, (rule, frag) ∈ frags -> (exists qi_rule, exists qf, regex2fragment rule.(Rule.regex) qi_rule = (qf, frag) /\ FRAGMENT_BOUNDS qi_rule qf frag /\ qi <= qi_rule /\ qf < qmax) ⟫.
+Proof.
+  revert qi qmax frags FRAGS.
+  induction rules as [ | rule' rules IH]; intros qi qmax frags FRAGS; simpl in FRAGS.
+  - inv FRAGS. split; [lia | intros rule frag IN; contradiction].
+  - destruct (regex2fragment rule'.(Rule.regex) qi) as [qf frag] eqn: REGEX2FRAGMENT.
+    destruct (rules2fragments (qf + 1) rules) as [qmax' frags'] eqn: FRAGS'.
+    injection FRAGS as Hqmax Hfrags. subst qmax frags.
+    pose proof (regex2fragment_bounds _ _ _ _ REGEX2FRAGMENT) as BOUNDS.
+    assert (LT : qi < qf) by (destruct BOUNDS as [_ _ LT _ _]; exact LT).
+    pose proof (IH (qf + 1) qmax' frags' FRAGS') as [QMAX TAIL].
+    split; [lia | intros rule frag' IN]. destruct IN as [EQ | IN].
+    + inv EQ. exists qi, qf. split; eauto. split; eauto. split; lia.
+    + pose proof (TAIL rule frag' IN) as (qi_rule & qf_rule & REGEX & BOUNDS' & LE_START & LT_END).
+      exists qi_rule, qf_rule. split; eauto. split; eauto. split; lia.
+Qed.
+
+Lemma rules2fragments_ranges_disjoint qi rules qmax frags rule1 frag1 qi1 qf1 rule2 frag2 qi2 qf2 q
+  (FRAGS : rules2fragments qi rules = (qmax, frags))
+  (IN1 : (rule1, frag1) ∈ frags)
+  (IN2 : (rule2, frag2) ∈ frags)
+  (REGEX1 : regex2fragment rule1.(Rule.regex) qi1 = (qf1, frag1))
+  (REGEX2 : regex2fragment rule2.(Rule.regex) qi2 = (qf2, frag2))
+  (RANGE1 : qi1 <= q <= qf1)
+  (RANGE2 : qi2 <= q <= qf2)
+  : (rule1, frag1) = (rule2, frag2).
+Proof.
+  revert qi qmax frags FRAGS rule1 frag1 qi1 qf1 rule2 frag2 qi2 qf2 q IN1 IN2 REGEX1 REGEX2 RANGE1 RANGE2.
+  induction rules as [ | rule rules IH]; ii.
+  - simpl in FRAGS. inv FRAGS. contradiction.
+  - simpl in FRAGS.
+    destruct (regex2fragment rule.(Rule.regex) qi) as [qf frag] eqn: REGEX.
+    destruct (rules2fragments (qf + 1) rules) as [qmax' frags'] eqn: FRAGS'.
+    injection FRAGS as Hqmax Hfrags. subst qmax frags.
+    pose proof (rules2fragments_bounds _ _ _ _ FRAGS') as [_ TAIL_BOUNDS].
+    destruct IN1 as [EQ1 | IN1]; destruct IN2 as [EQ2 | IN2].
+    + inv EQ1. inv EQ2. reflexivity.
+    + inv EQ1.
+      pose proof (regex2fragment_same_fragment _ _ _ _ _ _ REGEX1 REGEX) as [EQ_QI EQ_QF]. subst qi1 qf1.
+      pose proof (TAIL_BOUNDS _ _ IN2) as (qi2' & qf2' & REGEX2' & _ & LE2 & _).
+      pose proof (regex2fragment_same_fragment _ _ _ _ _ _ REGEX2 REGEX2') as [EQ_QI EQ_QF]. subst qi2 qf2.
+      lia.
+    + inv EQ2.
+      pose proof (regex2fragment_same_fragment _ _ _ _ _ _ REGEX2 REGEX) as [EQ_QI EQ_QF]. subst qi2 qf2.
+      pose proof (TAIL_BOUNDS _ _ IN1) as (qi1' & qf1' & REGEX1' & _ & LE1 & _).
+      pose proof (regex2fragment_same_fragment _ _ _ _ _ _ REGEX1 REGEX1') as [EQ_QI EQ_QF]. subst qi1 qf1.
+      lia.
+    + eapply IH; eauto.
+Qed.
+
+Lemma fragment_eps_edges_owner qi rules qmax frags q q'
+  (FRAGS : rules2fragments qi rules = (qmax, frags))
+  (IN_EDGE : (q, q') ∈ fragment_eps_edges frags)
+  (SRC_NONZERO : ~ q = 0)
+  : exists rule, exists frag, exists qi_rule, exists qf, (rule, frag) ∈ frags /\ regex2fragment rule.(Rule.regex) qi_rule = (qf, frag) /\ FRAGMENT_BOUNDS qi_rule qf frag /\ qi <= qi_rule /\ qf < qmax /\ qi_rule <= q <= qf /\ (q, q') ∈ frag.(frag_eps_edges).
+Proof.
+  revert qi qmax frags FRAGS IN_EDGE.
+  induction rules as [ | rule rules IH]; ii.
+  - simpl in FRAGS. inv FRAGS. contradiction.
+  - simpl in FRAGS.
+    destruct (regex2fragment rule.(Rule.regex) qi) as [qf frag] eqn: REGEX.
+    destruct (rules2fragments (qf + 1) rules) as [qmax' frags'] eqn: FRAGS'.
+    injection FRAGS as Hqmax Hfrags. subst qmax frags.
+    pose proof (rules2fragments_bounds _ _ _ _ FRAGS') as [QMAX _].
+    simpl in IN_EDGE. destruct IN_EDGE as [EQ | IN_EDGE].
+    + inv EQ. contradiction.
+    + rewrite in_app_iff in IN_EDGE. destruct IN_EDGE as [IN_EDGE | IN_EDGE].
+      * pose proof (regex2fragment_bounds _ _ _ _ REGEX) as BOUNDS.
+        destruct BOUNDS as [_ _ LT EPS _].
+        pose proof (EPS _ IN_EDGE). unfold eps_edge_in_range in *. simpl in *.
+        exists rule, frag, qi, qf. split; [left; reflexivity | ].
+        split; [exact REGEX | ]. split; [eapply regex2fragment_bounds; eauto | ].
+        split; [lia | ]. split; [lia | ]. split; [lia | exact IN_EDGE].
+      * pose proof (regex2fragment_bounds _ _ _ _ REGEX) as [_ _ LT _ _].
+        pose proof (IH (qf + 1) qmax' frags' FRAGS' IN_EDGE) as (rule' & frag' & qi_rule & qf' & IN_FRAG & REGEX' & BOUNDS & LE & LT' & RANGE & IN_EDGE').
+        exists rule', frag', qi_rule, qf'. split; [right; exact IN_FRAG | ].
+        split; [exact REGEX' | ]. split; [exact BOUNDS | ].
+        split; [lia | ]. split; [exact LT' | ]. split; [exact RANGE | exact IN_EDGE'].
+Qed.
+
+Lemma fragment_eps_edges_start_sound qi rules qmax frags q'
+  (FRAGS : rules2fragments qi rules = (qmax, frags))
+  (qi_POS : 0 < qi)
+  (IN_EDGE : (0, q') ∈ fragment_eps_edges frags)
+  : exists rule, exists frag, exists qi_rule, exists qf, (rule, frag) ∈ frags /\ regex2fragment rule.(Rule.regex) qi_rule = (qf, frag) /\ q' = frag.(frag_start).
+Proof.
+  revert qi qmax frags q' FRAGS qi_POS IN_EDGE.
+  induction rules as [ | rule rules IH]; ii; simpl in FRAGS.
+  - inv FRAGS. contradiction.
+  - destruct (regex2fragment rule.(Rule.regex) qi) as [qf frag] eqn: REGEX.
+    destruct (rules2fragments (qf + 1) rules) as [qmax' frags'] eqn: FRAGS'.
+    injection FRAGS as Hqmax Hfrags. subst qmax frags.
+    simpl in IN_EDGE. destruct IN_EDGE as [EQ | IN_EDGE].
+    + inv EQ. exists rule, frag, qi, qf. repeat split; eauto.
+      left. reflexivity.
+    + rewrite in_app_iff in IN_EDGE. destruct IN_EDGE as [IN_EDGE | IN_EDGE].
+      * pose proof (regex2fragment_bounds _ _ _ _ REGEX) as [_ _ _ EPS _].
+        pose proof (EPS _ IN_EDGE). unfold eps_edge_in_range in *. simpl in *. lia.
+      * pose proof (regex2fragment_bounds _ _ _ _ REGEX) as [_ _ LT _ _].
+        assert (qi_POS' : 0 < qf + 1) by lia.
+        pose proof (IH (qf + 1) qmax' frags' q' FRAGS' qi_POS' IN_EDGE) as (rule' & frag' & qi_rule & qf' & IN_FRAG & REGEX' & START).
+        exists rule', frag', qi_rule, qf'. split; [right; exact IN_FRAG | ].
+        split; [exact REGEX' | exact START].
+Qed.
+
+Lemma fragment_char_edges_owner qi rules qmax frags edge
+  (FRAGS : rules2fragments qi rules = (qmax, frags))
+  (IN_EDGE : edge ∈ fragment_char_edges frags)
+  : exists rule, exists frag, exists qi_rule, exists qf, (rule, frag) ∈ frags /\ regex2fragment rule.(Rule.regex) qi_rule = (qf, frag) /\ FRAGMENT_BOUNDS qi_rule qf frag /\ qi <= qi_rule /\ qf < qmax /\ qi_rule <= edge.(char_edge_src) <= qf /\ edge ∈ frag.(frag_char_edges).
+Proof.
+  revert qi qmax frags FRAGS IN_EDGE.
+  induction rules as [ | rule rules IH]; ii; simpl in FRAGS.
+  - inv FRAGS. contradiction.
+  - destruct (regex2fragment rule.(Rule.regex) qi) as [qf frag] eqn: REGEX.
+    destruct (rules2fragments (qf + 1) rules) as [qmax' frags'] eqn: FRAGS'.
+    injection FRAGS as Hqmax Hfrags. subst qmax frags.
+    pose proof (rules2fragments_bounds _ _ _ _ FRAGS') as [QMAX _].
+    simpl in IN_EDGE. rewrite in_app_iff in IN_EDGE. destruct IN_EDGE as [IN_EDGE | IN_EDGE].
+    + pose proof (regex2fragment_bounds _ _ _ _ REGEX) as BOUNDS.
+      destruct BOUNDS as [_ _ LT _ CHAR].
+      pose proof (CHAR _ IN_EDGE). unfold char_edge_in_range in *.
+      exists rule, frag, qi, qf. split; [left; reflexivity | ].
+      split; [exact REGEX | ]. split; [eapply regex2fragment_bounds; eauto | ].
+      repeat (split; [lia | eauto]).
+    + pose proof (regex2fragment_bounds _ _ _ _ REGEX) as [_ _ LT _ _].
+      pose proof (IH (qf + 1) qmax' frags' FRAGS' IN_EDGE) as (rule' & frag' & qi_rule & qf' & IN_FRAG & REGEX' & BOUNDS & LE & LT' & RANGE & IN_EDGE').
+      exists rule', frag', qi_rule, qf'. split; [right; exact IN_FRAG | ].
+      split; [exact REGEX' | ]. split; [exact BOUNDS | ].
+      repeat (split; [lia | eauto]).
+Qed.
+
+Lemma fragment_eps_edges_isolate qi rules qmax frags rule frag qi_rule qf q q'
+  (FRAGS : rules2fragments qi rules = (qmax, frags))
+  (IN_FRAG : (rule, frag) ∈ frags)
+  (REGEX : regex2fragment rule.(Rule.regex) qi_rule = (qf, frag))
+  (SRC_NONZERO : ~ q = 0)
+  (RANGE : qi_rule <= q <= qf)
+  (IN_EDGE : (q, q') ∈ fragment_eps_edges frags)
+  : (q, q') ∈ frag.(frag_eps_edges).
+Proof.
+  pose proof (fragment_eps_edges_owner _ _ _ _ _ _ FRAGS IN_EDGE SRC_NONZERO) as (rule' & frag' & qi_rule' & qf' & IN_FRAG' & REGEX' & _ & _ & _ & RANGE' & IN_EDGE').
+  pose proof (rules2fragments_ranges_disjoint _ _ _ _ _ _ _ _ _ _ _ _ _ FRAGS IN_FRAG IN_FRAG' REGEX REGEX' RANGE RANGE') as EQ.
+  inv EQ. exact IN_EDGE'.
+Qed.
+
+Lemma fragment_char_edges_isolate qi rules qmax frags rule frag qi_rule qf edge
+  (FRAGS : rules2fragments qi rules = (qmax, frags))
+  (IN_FRAG : (rule, frag) ∈ frags)
+  (REGEX : regex2fragment rule.(Rule.regex) qi_rule = (qf, frag))
+  (RANGE : qi_rule <= edge.(char_edge_src) <= qf)
+  (IN_EDGE : edge ∈ fragment_char_edges frags)
+  : edge ∈ frag.(frag_char_edges).
+Proof.
+  pose proof (fragment_char_edges_owner _ _ _ _ _ FRAGS IN_EDGE) as (rule' & frag' & qi_rule' & qf' & IN_FRAG' & REGEX' & _ & _ & _ & RANGE' & IN_EDGE').
+  pose proof (rules2fragments_ranges_disjoint _ _ _ _ _ _ _ _ _ _ _ _ _ FRAGS IN_FRAG IN_FRAG' REGEX REGEX' RANGE RANGE') as EQ.
+  inv EQ. exact IN_EDGE'.
+Qed.
+
+Lemma rules2fragments_start_ge qi rules qmax frags rule frag qi_rule qf
+  (FRAGS : rules2fragments qi rules = (qmax, frags))
+  (IN_FRAG : (rule, frag) ∈ frags)
+  (REGEX : regex2fragment rule.(Rule.regex) qi_rule = (qf, frag))
+  : qi <= qi_rule.
+Proof.
+  pose proof (rules2fragments_bounds _ _ _ _ FRAGS) as [_ BOUND].
+  pose proof (BOUND _ _ IN_FRAG) as (qi_rule' & qf' & REGEX' & _ & LE & _).
+  pose proof (regex2fragment_same_fragment _ _ _ _ _ _ REGEX REGEX') as [EQ _].
+  subst qi_rule'. exact LE.
+Qed.
+
+Lemma delta_star_fragment_range qi rules qmax frags rule frag qi_rule qf q q' s
+  (FRAGS : rules2fragments qi rules = (qmax, frags))
+  (IN_FRAG : (rule, frag) ∈ frags)
+  (REGEX : regex2fragment rule.(Rule.regex) qi_rule = (qf, frag))
+  (qi_POS : 0 < qi)
+  (RANGE : qi_rule <= q <= qf)
+  (DELTA : q' \in fragments_delta_star frags q s)
+  : qi_rule <= q' <= qf.
+Proof.
+  revert qi rules rule frag qi_rule qf FRAGS IN_FRAG REGEX qi_POS RANGE. induction DELTA; ii.
+  - exact RANGE.
+  - pose proof (eps_step_from_edges_sound _ _ _ STEP) as IN_EDGE.
+    assert (SRC_NONZERO : ~ q = 0) by (pose proof (rules2fragments_start_ge _ _ _ _ _ _ _ _ FRAGS IN_FRAG REGEX); lia).
+    pose proof (fragment_eps_edges_isolate _ _ _ _ _ _ _ _ _ _ FRAGS IN_FRAG REGEX SRC_NONZERO RANGE IN_EDGE) as IN_FRAG_EDGE.
+    pose proof (regex2fragment_bounds _ _ _ _ REGEX) as [_ _ _ EPS _].
+    pose proof (EPS _ IN_FRAG_EDGE). unfold eps_edge_in_range in *. simpl in *.
+    eapply IHDELTA; eauto. lia.
+  - pose proof (char_step_from_edges_sound _ _ _ _ STEP) as (edge & IN_EDGE & SRC & LABEL & DST).
+    assert (RANGE_SRC : qi_rule <= edge.(char_edge_src) <= qf) by lia.
+    pose proof (fragment_char_edges_isolate _ _ _ _ _ _ _ _ _ FRAGS IN_FRAG REGEX RANGE_SRC IN_EDGE) as IN_FRAG_EDGE.
+    pose proof (regex2fragment_bounds _ _ _ _ REGEX) as [_ _ _ _ CHAR].
+    pose proof (CHAR _ IN_FRAG_EDGE). unfold char_edge_in_range in *.
+    eapply IHDELTA; eauto. lia.
+Qed.
+
+Lemma delta_star_global_to_fragment qi rules qmax frags rule frag qi_rule qf q q' s
+  (FRAGS : rules2fragments qi rules = (qmax, frags))
+  (IN_FRAG : (rule, frag) ∈ frags)
+  (REGEX : regex2fragment rule.(Rule.regex) qi_rule = (qf, frag))
+  (qi_POS : 0 < qi)
+  (RANGE : qi_rule <= q <= qf)
+  (DELTA : q' \in fragments_delta_star frags q s)
+  : q' \in fragment_delta_star frag q s.
+Proof.
+  revert qi rules rule frag qi_rule qf FRAGS IN_FRAG REGEX qi_POS RANGE. induction DELTA; ii.
+  - econs.
+  - pose proof (eps_step_from_edges_sound _ _ _ STEP) as IN_EDGE.
+    assert (SRC_NONZERO : ~ q = 0) by (pose proof (rules2fragments_start_ge _ _ _ _ _ _ _ _ FRAGS IN_FRAG REGEX); lia).
+    pose proof (fragment_eps_edges_isolate _ _ _ _ _ _ _ _ _ _ FRAGS IN_FRAG REGEX SRC_NONZERO RANGE IN_EDGE) as IN_FRAG_EDGE.
+    pose proof (regex2fragment_bounds _ _ _ _ REGEX) as [_ _ _ EPS _].
+    pose proof (EPS _ IN_FRAG_EDGE). unfold eps_edge_in_range in *. simpl in *.
+    eapply delta_star_eps.
+    + eapply eps_step_from_edges_complete. exact IN_FRAG_EDGE.
+    + eapply IHDELTA; eauto. lia.
+  - pose proof (char_step_from_edges_sound _ _ _ _ STEP) as (edge & IN_EDGE & SRC & LABEL & DST).
+    assert (RANGE_SRC : qi_rule <= edge.(char_edge_src) <= qf) by lia.
+    pose proof (fragment_char_edges_isolate _ _ _ _ _ _ _ _ _ FRAGS IN_FRAG REGEX RANGE_SRC IN_EDGE) as IN_FRAG_EDGE.
+    pose proof (regex2fragment_bounds _ _ _ _ REGEX) as [_ _ _ _ CHAR].
+    pose proof (CHAR _ IN_FRAG_EDGE). unfold char_edge_in_range in *.
+    eapply delta_star_char with (q1 := edge.(char_edge_dst)).
+    + rewrite <- SRC. rewrite <- LABEL. eapply char_step_from_edges_complete. exact IN_FRAG_EDGE.
+    + rewrite DST. eapply IHDELTA; eauto. lia.
+Qed.
+
+Lemma regex2fragment_global_to_local qi rules qmax frags rule qf frag s
+  (FRAGS : rules2fragments qi rules = (qmax, frags))
+  (IN_FRAG : (rule, frag) ∈ frags)
+  (REGEX : regex2fragment rule.(Rule.regex) frag.(frag_start) = (qf, frag))
+  (qi_POS : 0 < qi)
+  (DELTA : frag.(frag_accept) \in fragments_delta_star frags frag.(frag_start) s)
+  : frag.(frag_accept) \in fragment_delta_star frag frag.(frag_start) s.
+Proof.
+  pose proof (regex2fragment_bounds _ _ _ _ REGEX) as [START ACCEPT LT _ _].
+  eapply delta_star_global_to_fragment; eauto. lia.
+Qed.
+
+Lemma delta_star_fragment_elim qi rules qmax frags rule frag qi_rule qf q q' s
+  (FRAGS : rules2fragments qi rules = (qmax, frags))
+  (IN_FRAG : (rule, frag) ∈ frags)
+  (REGEX : regex2fragment rule.(Rule.regex) qi_rule = (qf, frag))
+  (qi_POS : 0 < qi)
+  (RANGE : qi_rule <= q <= qf)
+  (DELTA : q' \in fragments_delta_star frags q s)
+  : ⟪ DELTA_STAR_NIL : s = [] /\ q' = q ⟫ \/ ⟪ DELTA_STAR_EPS : exists q1, (q, q1) ∈ frag.(frag_eps_edges) /\ q' \in fragments_delta_star frags q1 s ⟫ \/ ⟪ DELTA_STAR_CHAR : exists edge, exists s', s = edge.(char_edge_label) :: s' /\ edge ∈ frag.(frag_char_edges) /\ q' \in fragments_delta_star frags edge.(char_edge_dst) s' ⟫.
+Proof.
+  pose proof (delta_star_elim q q' s DELTA) as [NIL | [EPS | CHAR]].
+  - left. exact NIL.
+  - right. left. destruct EPS as (q1 & STEP & REST).
+    pose proof (eps_step_from_edges_sound _ _ _ STEP) as IN_EDGE.
+    assert (SRC_NONZERO : ~ q = 0) by (pose proof (rules2fragments_start_ge _ _ _ _ _ _ _ _ FRAGS IN_FRAG REGEX); lia).
+    pose proof (fragment_eps_edges_isolate _ _ _ _ _ _ _ _ _ _ FRAGS IN_FRAG REGEX SRC_NONZERO RANGE IN_EDGE) as IN_FRAG_EDGE.
+    exists q1. split; eauto.
+  - right. right. destruct CHAR as (c & s' & q1 & EQ & STEP & REST).
+    pose proof (char_step_from_edges_sound _ _ _ _ STEP) as (edge & IN_EDGE & SRC & LABEL & DST).
+    assert (RANGE_SRC : qi_rule <= edge.(char_edge_src) <= qf) by lia.
+    pose proof (fragment_char_edges_isolate _ _ _ _ _ _ _ _ _ FRAGS IN_FRAG REGEX RANGE_SRC IN_EDGE) as IN_FRAG_EDGE.
+    exists edge, s'. repeat split; eauto; try congruence.
+    now rewrite DST.
+Qed.
+
+Lemma fragment_delta_star_elim frag q q' s
+  (DELTA : q' \in fragment_delta_star frag q s)
+  : ⟪ DELTA_STAR_NIL : s = [] /\ q' = q ⟫ \/ ⟪ DELTA_STAR_EPS : exists q1, (q, q1) ∈ frag.(frag_eps_edges) /\ q' \in fragment_delta_star frag q1 s ⟫ \/ ⟪ DELTA_STAR_CHAR : exists edge, exists s', s = edge.(char_edge_label) :: s' /\ edge ∈ frag.(frag_char_edges) /\ q' \in fragment_delta_star frag edge.(char_edge_dst) s' ⟫.
+Proof.
+  pose proof (delta_star_elim q q' s DELTA) as [NIL | [EPS | CHAR]].
+  - left. exact NIL.
+  - right. left. destruct EPS as (q1 & STEP & REST).
+    pose proof (eps_step_from_edges_sound _ _ _ STEP). exists q1. eauto.
+  - right. right. destruct CHAR as (c & s' & q1 & EQ & STEP & REST).
+    pose proof (char_step_from_edges_sound _ _ _ _ STEP) as (edge & IN_EDGE & SRC & LABEL & DST).
+    exists edge, s'. repeat split; eauto; try congruence.
+    now rewrite DST.
+Qed.
+
+Lemma fragment_delta_star_elim_with_src frag q q' s
+  (DELTA : q' \in fragment_delta_star frag q s)
+  : ⟪ DELTA_STAR_NIL : s = [] /\ q' = q ⟫ \/ ⟪ DELTA_STAR_EPS : exists q1, (q, q1) ∈ frag.(frag_eps_edges) /\ q' \in fragment_delta_star frag q1 s ⟫ \/ ⟪ DELTA_STAR_CHAR : exists edge, exists s', s = edge.(char_edge_label) :: s' /\ edge.(char_edge_src) = q /\ edge ∈ frag.(frag_char_edges) /\ q' \in fragment_delta_star frag edge.(char_edge_dst) s' ⟫.
+Proof.
+  pose proof (delta_star_elim q q' s DELTA) as [NIL | [EPS | CHAR]].
+  - left. exact NIL.
+  - right. left. destruct EPS as (q1 & STEP & REST).
+    pose proof (eps_step_from_edges_sound _ _ _ STEP). exists q1. eauto.
+  - right. right. destruct CHAR as (c & s' & q1 & EQ & STEP & REST).
+    pose proof (char_step_from_edges_sound _ _ _ _ STEP) as (edge & IN_EDGE & SRC & LABEL & DST).
+    exists edge, s'. repeat split; eauto; try congruence.
+    now rewrite DST.
+Qed.
+
+Lemma regex2fragment_Union_delta_star_start qi qf frag e1 e2 s
+  (REGEX : regex2fragment (Re.Union e1 e2) qi = (qf, frag))
+  (DELTA : frag.(frag_accept) \in fragment_delta_star frag frag.(frag_start) s)
+  : exists qf1, exists frag1, exists qf2, exists frag2, regex2fragment e1 (qi + 1) = (qf1, frag1) /\ regex2fragment e2 (qf1 + 1) = (qf2, frag2) /\ (frag.(frag_accept) \in fragment_delta_star frag (qi + 1) s \/ frag.(frag_accept) \in fragment_delta_star frag (qf1 + 1) s).
+Proof.
+  simpl in REGEX. destruct (regex2fragment e1 (qi + 1)) as [qf1 frag1] eqn: REGEX1.
+  destruct (regex2fragment e2 (qf1 + 1)) as [qf2 frag2] eqn: REGEX2. inv REGEX.
+  exists qf1, frag1, qf2, frag2. repeat split; eauto.
+  pose proof (regex2fragment_bounds _ _ _ _ REGEX1) as [_ _ LT1 EPS1 CHAR1].
+  pose proof (regex2fragment_bounds _ _ _ _ REGEX2) as [_ _ LT2 EPS2 CHAR2].
+  pose proof (fragment_delta_star_elim_with_src _ _ _ _ DELTA) as [NIL | [EPS | CHAR]].
+  - des; simpl in *; lia.
+  - destruct EPS as (q1 & IN_EDGE & REST). simpl in IN_EDGE.
+    destruct IN_EDGE as [EQ | [EQ | [EQ | [EQ | IN_EDGE]]]].
+    + inv EQ. left. exact REST.
+    + inv EQ. right. exact REST.
+    + inv EQ. lia.
+    + inv EQ. lia.
+    + rewrite in_app_iff in IN_EDGE. destruct IN_EDGE as [IN_EDGE | IN_EDGE].
+      * pose proof (EPS1 _ IN_EDGE). unfold eps_edge_in_range in *. simpl in *. lia.
+      * pose proof (EPS2 _ IN_EDGE). unfold eps_edge_in_range in *. simpl in *. lia.
+  - destruct CHAR as (edge & s' & EQ & SRC & IN_EDGE & REST). simpl in IN_EDGE.
+    rewrite in_app_iff in IN_EDGE. destruct IN_EDGE as [IN_EDGE | IN_EDGE].
+    + pose proof (CHAR1 _ IN_EDGE) as [[SRC_LO SRC_HI] _].
+      simpl in SRC. exfalso. lia.
+    + pose proof (CHAR2 _ IN_EDGE) as [[SRC_LO SRC_HI] _].
+      simpl in SRC. exfalso. lia.
+Qed.
+
+Lemma regex2fragment_Union_left_delta_star_split qi qf frag e1 e2 qf1 frag1 qf2 frag2 q q' s
+  (REGEX : regex2fragment (Re.Union e1 e2) qi = (qf, frag))
+  (REGEX1 : regex2fragment e1 (qi + 1) = (qf1, frag1))
+  (REGEX2 : regex2fragment e2 (qf1 + 1) = (qf2, frag2))
+  (RANGE : qi + 1 <= q <= qf1)
+  (DELTA : q' \in fragment_delta_star frag q s)
+  (ACCEPT : q' = frag.(frag_accept))
+  : exists s1, exists s2, s = s1 ++ s2 /\ qf1 \in fragment_delta_star frag1 q s1 /\ frag.(frag_accept) \in fragment_delta_star frag frag.(frag_accept) s2.
+Proof.
+  revert q q' s RANGE DELTA ACCEPT.
+  simpl in REGEX. rewrite REGEX1 in REGEX. rewrite REGEX2 in REGEX. inv REGEX.
+  intros q q' s RANGE DELTA ACCEPT.
+  pose proof (regex2fragment_bounds _ _ _ _ REGEX1) as [_ _ LT1 EPS1 CHAR1].
+  pose proof (regex2fragment_bounds _ _ _ _ REGEX2) as [_ _ LT2 EPS2 CHAR2].
+  revert RANGE ACCEPT. induction DELTA; intros RANGE ACCEPT.
+  - simpl in *. lia.
+  - pose proof (eps_step_from_edges_sound _ _ _ STEP) as IN_EDGE. simpl in IN_EDGE.
+    destruct IN_EDGE as [EQ | [EQ | [EQ | [EQ | IN_EDGE]]]].
+    + injection EQ as EQ1 EQ2. lia.
+    + injection EQ as EQ1 EQ2. lia.
+    + injection EQ as EQ1 EQ2. subst q q1. exists [], s. repeat split; eauto.
+      * econs.
+      * now rewrite ACCEPT in REST.
+    + injection EQ as EQ1 EQ2. lia.
+    + rewrite in_app_iff in IN_EDGE. destruct IN_EDGE as [IN_EDGE | IN_EDGE].
+      * pose proof (EPS1 _ IN_EDGE) as [[SRC_LO SRC_HI] [DST_LO DST_HI]].
+        simpl in SRC_LO, SRC_HI, DST_LO, DST_HI.
+        assert (RANGE_STEP : qi + 1 <= q1 <= qf1) by lia.
+        pose proof (IHDELTA RANGE_STEP ACCEPT) as (s1 & s2 & EQ & DELTA1 & DELTA2).
+        exists s1, s2. repeat split; eauto.
+        eapply delta_star_eps; eauto. eapply eps_step_from_edges_complete. exact IN_EDGE.
+      * pose proof (EPS2 _ IN_EDGE) as [[SRC_LO SRC_HI] _]. simpl in *. lia.
+  - pose proof (char_step_from_edges_sound _ _ _ _ STEP) as (edge & IN_EDGE & SRC & LABEL & DST).
+    simpl in IN_EDGE. rewrite in_app_iff in IN_EDGE. destruct IN_EDGE as [IN_EDGE | IN_EDGE].
+    + pose proof (CHAR1 _ IN_EDGE) as [[SRC_LO SRC_HI] [DST_LO DST_HI]].
+      assert (RANGE_STEP : qi + 1 <= q1 <= qf1) by lia.
+      pose proof (IHDELTA RANGE_STEP ACCEPT) as (s1 & s2 & EQ & DELTA1 & DELTA2).
+      exists (edge.(char_edge_label) :: s1), s2. split.
+      * rewrite EQ. simpl. now rewrite LABEL.
+      * split; eauto. eapply delta_star_char with (q1 := q1).
+        { rewrite <- DST. rewrite <- SRC. eapply char_step_from_edges_complete. exact IN_EDGE. }
+        { exact DELTA1. }
+    + pose proof (CHAR2 _ IN_EDGE) as [[SRC_LO SRC_HI] _]. simpl in SRC. lia.
+Qed.
+
+Lemma regex2fragment_Union_right_delta_star_split qi qf frag e1 e2 qf1 frag1 qf2 frag2 q q' s
+  (REGEX : regex2fragment (Re.Union e1 e2) qi = (qf, frag))
+  (REGEX1 : regex2fragment e1 (qi + 1) = (qf1, frag1))
+  (REGEX2 : regex2fragment e2 (qf1 + 1) = (qf2, frag2))
+  (RANGE : qf1 + 1 <= q <= qf2)
+  (DELTA : q' \in fragment_delta_star frag q s)
+  (ACCEPT : q' = frag.(frag_accept))
+  : exists s1, exists s2, s = s1 ++ s2 /\ qf2 \in fragment_delta_star frag2 q s1 /\ frag.(frag_accept) \in fragment_delta_star frag frag.(frag_accept) s2.
+Proof.
+  revert q q' s RANGE DELTA ACCEPT.
+  simpl in REGEX. rewrite REGEX1 in REGEX. rewrite REGEX2 in REGEX. inv REGEX.
+  intros q q' s RANGE DELTA ACCEPT.
+  pose proof (regex2fragment_bounds _ _ _ _ REGEX1) as [_ _ LT1 EPS1 CHAR1].
+  pose proof (regex2fragment_bounds _ _ _ _ REGEX2) as [_ _ LT2 EPS2 CHAR2].
+  revert RANGE ACCEPT. induction DELTA; intros RANGE ACCEPT.
+  - simpl in *. lia.
+  - pose proof (eps_step_from_edges_sound _ _ _ STEP) as IN_EDGE. simpl in IN_EDGE.
+    destruct IN_EDGE as [EQ | [EQ | [EQ | [EQ | IN_EDGE]]]].
+    + injection EQ as EQ1 EQ2. lia.
+    + injection EQ as EQ1 EQ2. lia.
+    + injection EQ as EQ1 EQ2. lia.
+    + injection EQ as EQ1 EQ2. subst q q1. exists [], s. repeat split; eauto.
+      * econs.
+      * now rewrite ACCEPT in REST.
+    + rewrite in_app_iff in IN_EDGE. destruct IN_EDGE as [IN_EDGE | IN_EDGE].
+      * pose proof (EPS1 _ IN_EDGE) as [[SRC_LO SRC_HI] _]. simpl in *. lia.
+      * pose proof (EPS2 _ IN_EDGE) as [[SRC_LO SRC_HI] [DST_LO DST_HI]].
+        simpl in SRC_LO, SRC_HI, DST_LO, DST_HI.
+        assert (RANGE_STEP : qf1 + 1 <= q1 <= qf2) by lia.
+        pose proof (IHDELTA RANGE_STEP ACCEPT) as (s1 & s2 & EQ & DELTA1 & DELTA2).
+        exists s1, s2. repeat split; eauto.
+        eapply delta_star_eps; eauto. eapply eps_step_from_edges_complete. exact IN_EDGE.
+  - pose proof (char_step_from_edges_sound _ _ _ _ STEP) as (edge & IN_EDGE & SRC & LABEL & DST).
+    simpl in IN_EDGE. rewrite in_app_iff in IN_EDGE. destruct IN_EDGE as [IN_EDGE | IN_EDGE].
+    + pose proof (CHAR1 _ IN_EDGE) as [[SRC_LO SRC_HI] _]. simpl in SRC. lia.
+    + pose proof (CHAR2 _ IN_EDGE) as [[SRC_LO SRC_HI] [DST_LO DST_HI]].
+      assert (RANGE_STEP : qf1 + 1 <= q1 <= qf2) by lia.
+      pose proof (IHDELTA RANGE_STEP ACCEPT) as (s1 & s2 & EQ & DELTA1 & DELTA2).
+      exists (edge.(char_edge_label) :: s1), s2. split.
+      * rewrite EQ. simpl. now rewrite LABEL.
+      * split; eauto. eapply delta_star_char with (q1 := q1).
+        { rewrite <- DST. rewrite <- SRC. eapply char_step_from_edges_complete. exact IN_EDGE. }
+        { exact DELTA1. }
+Qed.
+
+Lemma regex2fragment_Append_delta_star_start qi qf frag e1 e2 s
+  (REGEX : regex2fragment (Re.Append e1 e2) qi = (qf, frag))
+  (DELTA : frag.(frag_accept) \in fragment_delta_star frag frag.(frag_start) s)
+  : exists qf1, exists frag1, exists qf2, exists frag2, regex2fragment e1 (qi + 1) = (qf1, frag1) /\ regex2fragment e2 (qf1 + 1) = (qf2, frag2) /\ frag.(frag_accept) \in fragment_delta_star frag (qi + 1) s.
+Proof.
+  simpl in REGEX. destruct (regex2fragment e1 (qi + 1)) as [qf1 frag1] eqn: REGEX1.
+  destruct (regex2fragment e2 (qf1 + 1)) as [qf2 frag2] eqn: REGEX2. inv REGEX.
+  exists qf1, frag1, qf2, frag2. repeat split; eauto.
+  pose proof (regex2fragment_bounds _ _ _ _ REGEX1) as [_ _ LT1 EPS1 CHAR1].
+  pose proof (regex2fragment_bounds _ _ _ _ REGEX2) as [_ _ LT2 EPS2 CHAR2].
+  pose proof (fragment_delta_star_elim_with_src _ _ _ _ DELTA) as [NIL | [EPS | CHAR]].
+  - des; simpl in *; lia.
+  - destruct EPS as (q1 & IN_EDGE & REST). simpl in IN_EDGE.
+    destruct IN_EDGE as [EQ | [EQ | [EQ | IN_EDGE]]].
+    + inv EQ. exact REST.
+    + inv EQ. lia.
+    + inv EQ. lia.
+    + rewrite in_app_iff in IN_EDGE. destruct IN_EDGE as [IN_EDGE | IN_EDGE].
+      * pose proof (EPS1 _ IN_EDGE). unfold eps_edge_in_range in *. simpl in *. lia.
+      * pose proof (EPS2 _ IN_EDGE). unfold eps_edge_in_range in *. simpl in *. lia.
+  - destruct CHAR as (edge & s' & EQ & SRC & IN_EDGE & REST). simpl in IN_EDGE.
+    rewrite in_app_iff in IN_EDGE. destruct IN_EDGE as [IN_EDGE | IN_EDGE].
+    + pose proof (CHAR1 _ IN_EDGE) as [[SRC_LO SRC_HI] _].
+      simpl in SRC. exfalso. lia.
+    + pose proof (CHAR2 _ IN_EDGE) as [[SRC_LO SRC_HI] _].
+      simpl in SRC. exfalso. lia.
+Qed.
+
+Lemma regex2fragment_Append_left_delta_star_split qi qf frag e1 e2 qf1 frag1 qf2 frag2 q q' s
+  (REGEX : regex2fragment (Re.Append e1 e2) qi = (qf, frag))
+  (REGEX1 : regex2fragment e1 (qi + 1) = (qf1, frag1))
+  (REGEX2 : regex2fragment e2 (qf1 + 1) = (qf2, frag2))
+  (RANGE : qi + 1 <= q <= qf1)
+  (DELTA : q' \in fragment_delta_star frag q s)
+  (ACCEPT : q' = frag.(frag_accept))
+  : exists s1, exists s2, s = s1 ++ s2 /\ qf1 \in fragment_delta_star frag1 q s1 /\ frag.(frag_accept) \in fragment_delta_star frag (qf1 + 1) s2.
+Proof.
+  revert q q' s RANGE DELTA ACCEPT.
+  simpl in REGEX. rewrite REGEX1 in REGEX. rewrite REGEX2 in REGEX. inv REGEX.
+  intros q q' s RANGE DELTA ACCEPT.
+  pose proof (regex2fragment_bounds _ _ _ _ REGEX1) as [_ _ LT1 EPS1 CHAR1].
+  pose proof (regex2fragment_bounds _ _ _ _ REGEX2) as [_ _ LT2 EPS2 CHAR2].
+  revert RANGE ACCEPT. induction DELTA; intros RANGE ACCEPT.
+  - simpl in *. lia.
+  - pose proof (eps_step_from_edges_sound _ _ _ STEP) as IN_EDGE. simpl in IN_EDGE.
+    destruct IN_EDGE as [EQ | [EQ | [EQ | IN_EDGE]]].
+    + injection EQ as EQ1 EQ2. lia.
+    + injection EQ as EQ1 EQ2. subst q q1. exists [], s. repeat split; eauto.
+      * econs.
+      * now rewrite ACCEPT in REST.
+    + injection EQ as EQ1 EQ2. lia.
+    + rewrite in_app_iff in IN_EDGE. destruct IN_EDGE as [IN_EDGE | IN_EDGE].
+      * pose proof (EPS1 _ IN_EDGE) as [[SRC_LO SRC_HI] [DST_LO DST_HI]].
+        simpl in SRC_LO, SRC_HI, DST_LO, DST_HI.
+        assert (RANGE_STEP : qi + 1 <= q1 <= qf1) by lia.
+        pose proof (IHDELTA RANGE_STEP ACCEPT) as (s1 & s2 & EQ & DELTA1 & DELTA2).
+        exists s1, s2. repeat split; eauto.
+        eapply delta_star_eps; eauto. eapply eps_step_from_edges_complete. exact IN_EDGE.
+      * pose proof (EPS2 _ IN_EDGE) as [[SRC_LO SRC_HI] _]. simpl in *. lia.
+  - pose proof (char_step_from_edges_sound _ _ _ _ STEP) as (edge & IN_EDGE & SRC & LABEL & DST).
+    simpl in IN_EDGE. rewrite in_app_iff in IN_EDGE. destruct IN_EDGE as [IN_EDGE | IN_EDGE].
+    + pose proof (CHAR1 _ IN_EDGE) as [[SRC_LO SRC_HI] [DST_LO DST_HI]].
+      assert (RANGE_STEP : qi + 1 <= q1 <= qf1) by lia.
+      pose proof (IHDELTA RANGE_STEP ACCEPT) as (s1 & s2 & EQ & DELTA1 & DELTA2).
+      exists (edge.(char_edge_label) :: s1), s2. split.
+      * rewrite EQ. simpl. now rewrite LABEL.
+      * split; eauto. eapply delta_star_char with (q1 := q1).
+        { rewrite <- DST. rewrite <- SRC. eapply char_step_from_edges_complete. exact IN_EDGE. }
+        { exact DELTA1. }
+    + pose proof (CHAR2 _ IN_EDGE) as [[SRC_LO SRC_HI] _]. simpl in SRC. lia.
+Qed.
+
+Lemma regex2fragment_Append_right_delta_star_split qi qf frag e1 e2 qf1 frag1 qf2 frag2 q q' s
+  (REGEX : regex2fragment (Re.Append e1 e2) qi = (qf, frag))
+  (REGEX1 : regex2fragment e1 (qi + 1) = (qf1, frag1))
+  (REGEX2 : regex2fragment e2 (qf1 + 1) = (qf2, frag2))
+  (RANGE : qf1 + 1 <= q <= qf2)
+  (DELTA : q' \in fragment_delta_star frag q s)
+  (ACCEPT : q' = frag.(frag_accept))
+  : exists s1, exists s2, s = s1 ++ s2 /\ qf2 \in fragment_delta_star frag2 q s1 /\ frag.(frag_accept) \in fragment_delta_star frag frag.(frag_accept) s2.
+Proof.
+  revert q q' s RANGE DELTA ACCEPT.
+  simpl in REGEX. rewrite REGEX1 in REGEX. rewrite REGEX2 in REGEX. inv REGEX.
+  intros q q' s RANGE DELTA ACCEPT.
+  pose proof (regex2fragment_bounds _ _ _ _ REGEX1) as [_ _ LT1 EPS1 CHAR1].
+  pose proof (regex2fragment_bounds _ _ _ _ REGEX2) as [_ _ LT2 EPS2 CHAR2].
+  revert RANGE ACCEPT. induction DELTA; intros RANGE ACCEPT.
+  - simpl in *. lia.
+  - pose proof (eps_step_from_edges_sound _ _ _ STEP) as IN_EDGE. simpl in IN_EDGE.
+    destruct IN_EDGE as [EQ | [EQ | [EQ | IN_EDGE]]].
+    + injection EQ as EQ1 EQ2. lia.
+    + injection EQ as EQ1 EQ2. lia.
+    + injection EQ as EQ1 EQ2. subst q q1. exists [], s. repeat split; eauto.
+      * econs.
+      * now rewrite ACCEPT in REST.
+    + rewrite in_app_iff in IN_EDGE. destruct IN_EDGE as [IN_EDGE | IN_EDGE].
+      * pose proof (EPS1 _ IN_EDGE) as [[SRC_LO SRC_HI] _]. simpl in *. lia.
+      * pose proof (EPS2 _ IN_EDGE) as [[SRC_LO SRC_HI] [DST_LO DST_HI]].
+        simpl in SRC_LO, SRC_HI, DST_LO, DST_HI.
+        assert (RANGE_STEP : qf1 + 1 <= q1 <= qf2) by lia.
+        pose proof (IHDELTA RANGE_STEP ACCEPT) as (s1 & s2 & EQ & DELTA1 & DELTA2).
+        exists s1, s2. repeat split; eauto.
+        eapply delta_star_eps; eauto. eapply eps_step_from_edges_complete. exact IN_EDGE.
+  - pose proof (char_step_from_edges_sound _ _ _ _ STEP) as (edge & IN_EDGE & SRC & LABEL & DST).
+    simpl in IN_EDGE. rewrite in_app_iff in IN_EDGE. destruct IN_EDGE as [IN_EDGE | IN_EDGE].
+    + pose proof (CHAR1 _ IN_EDGE) as [[SRC_LO SRC_HI] _]. simpl in SRC. lia.
+    + pose proof (CHAR2 _ IN_EDGE) as [[SRC_LO SRC_HI] [DST_LO DST_HI]].
+      assert (RANGE_STEP : qf1 + 1 <= q1 <= qf2) by lia.
+      pose proof (IHDELTA RANGE_STEP ACCEPT) as (s1 & s2 & EQ & DELTA1 & DELTA2).
+      exists (edge.(char_edge_label) :: s1), s2. split.
+      * rewrite EQ. simpl. now rewrite LABEL.
+      * split; eauto. eapply delta_star_char with (q1 := q1).
+        { rewrite <- DST. rewrite <- SRC. eapply char_step_from_edges_complete. exact IN_EDGE. }
+        { exact DELTA1. }
+Qed.
+
+Lemma regex2fragment_Star_delta_star_start qi qf frag e s
+  (REGEX : regex2fragment (Re.Star e) qi = (qf, frag))
+  (DELTA : frag.(frag_accept) \in fragment_delta_star frag frag.(frag_start) s)
+  : exists qf1, exists frag1, regex2fragment e (qi + 1) = (qf1, frag1) /\ frag.(frag_accept) \in fragment_delta_star frag (qi + 1) s.
+Proof.
+  simpl in REGEX. destruct (regex2fragment e (qi + 1)) as [qf1 frag1] eqn: REGEX1.
+  inv REGEX. exists qf1, frag1. split; eauto.
+  pose proof (regex2fragment_bounds _ _ _ _ REGEX1) as [_ _ LT1 EPS1 CHAR1].
+  pose proof (fragment_delta_star_elim_with_src _ _ _ _ DELTA) as [NIL | [EPS | CHAR]].
+  - des; simpl in *; lia.
+  - destruct EPS as (q1 & IN_EDGE & REST). simpl in IN_EDGE.
+    destruct IN_EDGE as [EQ | [EQ | [EQ | IN_EDGE]]].
+    + inv EQ. exact REST.
+    + inv EQ. lia.
+    + inv EQ. lia.
+    + pose proof (EPS1 _ IN_EDGE). unfold eps_edge_in_range in *. simpl in *. lia.
+  - destruct CHAR as (edge & s' & EQ & SRC & IN_EDGE & REST).
+    pose proof (CHAR1 _ IN_EDGE) as [[SRC_LO SRC_HI] _].
+    simpl in SRC. exfalso. lia.
+Qed.
+
+Lemma regex2fragment_accept_delta_star_stuck e qi qf frag q' s
+  (REGEX : regex2fragment e qi = (qf, frag))
+  (DELTA : q' \in fragment_delta_star frag qf s)
+  : s = [] /\ q' = qf.
+Proof.
+  eapply delta_star_stuck; eauto.
+  - intros q IN. pose proof (eps_step_from_edges_sound _ _ _ IN) as IN_EDGE.
+    pose proof (regex2fragment_edge_src_lt _ _ _ _ REGEX) as [EPS _].
+    pose proof (EPS _ _ IN_EDGE). lia.
+  - intros c q IN. pose proof (char_step_from_edges_sound _ _ _ _ IN) as (edge & IN_EDGE & SRC & LABEL & DST).
+    pose proof (regex2fragment_edge_src_lt _ _ _ _ REGEX) as [_ CHAR].
+    pose proof (CHAR _ IN_EDGE). lia.
+Qed.
+
+Lemma regex2fragment_Star_delta_star_sound_aux e
+  (SOUND : forall qi, forall qf, forall frag, forall s, regex2fragment e qi = (qf, frag) -> frag.(frag_accept) \in fragment_delta_star frag frag.(frag_start) s -> s \in eval_regex e)
+  : forall qi, forall qf, forall frag, forall qf1, forall frag1, forall q, forall q', forall s, regex2fragment (Re.Star e) qi = (qf, frag) -> regex2fragment e (qi + 1) = (qf1, frag1) -> qi + 1 <= q <= qf1 -> q' \in fragment_delta_star frag q s -> q' = frag.(frag_accept) ->  ((s = [] /\ q = qi + 1) \/ (exists s1, exists s2, s = s1 ++ s2 /\ qf1 \in fragment_delta_star frag1 q s1 /\ s2 \in eval_regex (Re.Star e))).
+Proof.
+  ii. revert q q' s H1 H2 H3.
+  simpl in H. rewrite H0 in H. inv H.
+  intros q q' s RANGE DELTA ACCEPT.
+  pose proof (regex2fragment_bounds _ _ _ _ H0) as [START1 ACCEPT1 LT1 EPS1 CHAR1].
+  pose proof (regex2fragment_edge_dst_gt_start _ _ _ _ H0) as [EPS_DST CHAR_DST].
+  revert RANGE ACCEPT. induction DELTA; intros RANGE ACCEPT.
+  - simpl in *. lia.
+  - pose proof (eps_step_from_edges_sound _ _ _ STEP) as IN_EDGE. simpl in IN_EDGE.
+    destruct IN_EDGE as [EQ | [EQ | [EQ | IN_EDGE]]].
+    + injection EQ as EQ1 EQ2. lia.
+    + injection EQ as EQ1 EQ2. subst q q1.
+      assert (STAR_IN : s \in eval_regex (Re.Star e)).
+      { assert (RANGE_STEP : qi + 1 <= qi + 1 <= qf1) by lia.
+        pose proof (IHDELTA RANGE_STEP ACCEPT) as [[EQ _] | (s1 & s2 & EQ & DELTA1 & STAR)].
+        - subst s. simpl. econs.
+        - subst s. simpl. eapply star_app.
+          + eapply SOUND; eauto. rewrite START1. rewrite ACCEPT1. exact DELTA1.
+          + exact STAR.
+      }
+      right. exists [], s. repeat split; eauto. econs.
+    + injection EQ as EQ1 EQ2. subst q q1.
+      assert (REGEX_STAR : regex2fragment (Re.Star e) qi = (qf1 + 1, mkFragment qi (qf1 + 1) ((qi, qi + 1) :: (qf1, qi + 1) :: (qi + 1, qf1 + 1) :: frag1.(frag_eps_edges)) frag1.(frag_char_edges))) by (simpl; rewrite H0; reflexivity).
+      pose proof (regex2fragment_accept_delta_star_stuck (Re.Star e) qi (qf1 + 1) (mkFragment qi (qf1 + 1) ((qi, qi + 1) :: (qf1, qi + 1) :: (qi + 1, qf1 + 1) :: frag1.(frag_eps_edges)) frag1.(frag_char_edges)) q2 s REGEX_STAR REST) as [EQ _].
+      subst s. left. split; eauto.
+    + pose proof (EPS1 _ IN_EDGE) as [[SRC_LO SRC_HI] [DST_LO DST_HI]].
+      simpl in SRC_LO, SRC_HI, DST_LO, DST_HI.
+      assert (RANGE_STEP : qi + 1 <= q1 <= qf1) by lia.
+      pose proof (IHDELTA RANGE_STEP ACCEPT) as [[EQ EQ'] | (s1 & s2 & EQ & DELTA1 & STAR)].
+      * subst s q1. pose proof (EPS_DST _ _ IN_EDGE). lia.
+      * right. exists s1, s2. repeat split; eauto.
+        eapply delta_star_eps; eauto. eapply eps_step_from_edges_complete. exact IN_EDGE.
+  - pose proof (char_step_from_edges_sound _ _ _ _ STEP) as (edge & IN_EDGE & SRC & LABEL & DST).
+    pose proof (CHAR1 _ IN_EDGE) as [[SRC_LO SRC_HI] [DST_LO DST_HI]].
+    assert (RANGE_STEP : qi + 1 <= q1 <= qf1) by lia.
+    pose proof (IHDELTA RANGE_STEP ACCEPT) as [[EQ EQ'] | (s1 & s2 & EQ & DELTA1 & STAR)].
+    + subst s q1. pose proof (CHAR_DST _ IN_EDGE). lia.
+    + right. exists (edge.(char_edge_label) :: s1), s2. split.
+      * rewrite EQ. simpl. now rewrite LABEL.
+      * split; eauto. eapply delta_star_char with (q1 := q1).
+        { rewrite <- DST. rewrite <- SRC. eapply char_step_from_edges_complete. exact IN_EDGE. }
+        { exact DELTA1. }
+Qed.
+
+Theorem regex2fragment_sound_Null qi qf frag s
+  (REGEX : regex2fragment Re.Null qi = (qf, frag))
+  (DELTA : frag.(frag_accept) \in fragment_delta_star frag frag.(frag_start) s)
+  : s \in eval_regex Re.Null.
+Proof.
+  simpl in REGEX. inv REGEX. pose proof (fragment_delta_star_elim _ _ _ _ DELTA) as [NIL | [EPS | CHAR]].
+  - des; simpl in *; lia.
+  - des; contradiction.
+  - des; contradiction.
+Qed.
+
+Theorem regex2fragment_sound_Empty qi qf frag s
+  (REGEX : regex2fragment Re.Empty qi = (qf, frag))
+  (DELTA : frag.(frag_accept) \in fragment_delta_star frag frag.(frag_start) s)
+  : s \in eval_regex Re.Empty.
+Proof.
+  simpl in REGEX. inv REGEX. pose proof (fragment_delta_star_elim _ _ _ _ DELTA) as [NIL | [EPS | CHAR]].
+  - des; simpl in *; lia.
+  - destruct EPS as (q1 & IN_EDGE & REST). simpl in IN_EDGE.
+    destruct IN_EDGE as [EQ | []]. inv EQ.
+    pose proof (regex2fragment_accept_delta_star_stuck Re.Empty qi (qi + 1) (mkFragment qi (qi + 1) [(qi, qi + 1)] []) (qi + 1) s eq_refl REST) as [EQ ?].
+    subst s. simpl. autorewrite with simplication_hints. reflexivity.
+  - des; contradiction.
+Qed.
+
+Theorem regex2fragment_sound_Char c qi qf frag s
+  (REGEX : regex2fragment (Re.Char c) qi = (qf, frag))
+  (DELTA : frag.(frag_accept) \in fragment_delta_star frag frag.(frag_start) s)
+  : s \in eval_regex (Re.Char c).
+Proof.
+  simpl in REGEX. inv REGEX. pose proof (fragment_delta_star_elim _ _ _ _ DELTA) as [NIL | [EPS | CHAR]].
+  - des; simpl in *; lia.
+  - des; contradiction.
+  - destruct CHAR as (edge & s' & EQ & IN_EDGE & REST). simpl in IN_EDGE.
+    destruct IN_EDGE as [EDGE_EQ | []]. subst edge. simpl in EQ. subst s.
+    pose proof (regex2fragment_accept_delta_star_stuck (Re.Char c) qi (qi + 1) (mkFragment qi (qi + 1) [] [mkCharEdge qi c (qi + 1)]) (qi + 1) s' eq_refl REST) as [EQ ?].
+    subst s'. simpl. autorewrite with simplication_hints. reflexivity.
+Qed.
+
+Theorem regex2fragment_sound_Union e1 e2
+  (SOUND1 : forall qi, forall qf, forall frag, forall s, regex2fragment e1 qi = (qf, frag) -> frag.(frag_accept) \in fragment_delta_star frag frag.(frag_start) s -> s \in eval_regex e1)
+  (SOUND2 : forall qi, forall qf, forall frag, forall s, regex2fragment e2 qi = (qf, frag) -> frag.(frag_accept) \in fragment_delta_star frag frag.(frag_start) s -> s \in eval_regex e2)
+  : forall qi, forall qf, forall frag, forall s, regex2fragment (Re.Union e1 e2) qi = (qf, frag) -> frag.(frag_accept) \in fragment_delta_star frag frag.(frag_start) s -> s \in eval_regex (Re.Union e1 e2).
+Proof.
+  ii. pose proof (regex2fragment_start_accept _ _ _ _ H) as [_ ACCEPT].
+  pose proof (regex2fragment_Union_delta_star_start qi qf frag e1 e2 s H H0) as (qf1 & frag1 & qf2 & frag2 & REGEX1 & REGEX2 & [DELTA1 | DELTA2]).
+  - pose proof (regex2fragment_bounds _ _ _ _ REGEX1) as [START1 ACCEPT1 LT1 _ _].
+    assert (RANGE1 : qi + 1 <= qi + 1 <= qf1) by lia.
+    pose proof (regex2fragment_Union_left_delta_star_split qi qf frag e1 e2 qf1 frag1 qf2 frag2 (qi + 1) frag.(frag_accept) s H REGEX1 REGEX2 RANGE1 DELTA1 eq_refl) as (s1 & s2 & EQ & DELTA1' & DELTA2').
+    rewrite ACCEPT in DELTA2'.
+    pose proof (regex2fragment_accept_delta_star_stuck (Re.Union e1 e2) qi qf frag qf s2 H DELTA2') as [EQ2 _].
+    subst s2. rewrite app_nil_r in EQ. subst s.
+    simpl. rewrite E.in_union_iff. left. eapply SOUND1; eauto.
+    rewrite START1. rewrite ACCEPT1. exact DELTA1'.
+  - pose proof (regex2fragment_bounds _ _ _ _ REGEX2) as [START2 ACCEPT2 LT2 _ _].
+    assert (RANGE2 : qf1 + 1 <= qf1 + 1 <= qf2) by lia.
+    pose proof (regex2fragment_Union_right_delta_star_split qi qf frag e1 e2 qf1 frag1 qf2 frag2 (qf1 + 1) frag.(frag_accept) s H REGEX1 REGEX2 RANGE2 DELTA2 eq_refl) as (s1 & s2 & EQ & DELTA1' & DELTA2').
+    rewrite ACCEPT in DELTA2'.
+    pose proof (regex2fragment_accept_delta_star_stuck (Re.Union e1 e2) qi qf frag qf s2 H DELTA2') as [EQ2 _].
+    subst s2. rewrite app_nil_r in EQ. subst s.
+    simpl. rewrite E.in_union_iff. right. eapply SOUND2; eauto.
+    rewrite START2. rewrite ACCEPT2. exact DELTA1'.
+Qed.
+
+Theorem regex2fragment_sound_Append e1 e2
+  (SOUND1 : forall qi, forall qf, forall frag, forall s, regex2fragment e1 qi = (qf, frag) -> frag.(frag_accept) \in fragment_delta_star frag frag.(frag_start) s -> s \in eval_regex e1)
+  (SOUND2 : forall qi, forall qf, forall frag, forall s, regex2fragment e2 qi = (qf, frag) -> frag.(frag_accept) \in fragment_delta_star frag frag.(frag_start) s -> s \in eval_regex e2)
+  : forall qi, forall qf, forall frag, forall s, regex2fragment (Re.Append e1 e2) qi = (qf, frag) -> frag.(frag_accept) \in fragment_delta_star frag frag.(frag_start) s -> s \in eval_regex (Re.Append e1 e2).
+Proof.
+  ii. pose proof (regex2fragment_start_accept _ _ _ _ H) as [_ ACCEPT].
+  pose proof (regex2fragment_Append_delta_star_start qi qf frag e1 e2 s H H0) as (qf1 & frag1 & qf2 & frag2 & REGEX1 & REGEX2 & DELTA).
+  pose proof (regex2fragment_bounds _ _ _ _ REGEX1) as [START1 ACCEPT1 LT1 _ _].
+  pose proof (regex2fragment_bounds _ _ _ _ REGEX2) as [START2 ACCEPT2 LT2 _ _].
+  assert (RANGE1 : qi + 1 <= qi + 1 <= qf1) by lia.
+  assert (RANGE2 : qf1 + 1 <= qf1 + 1 <= qf2) by lia.
+  pose proof (regex2fragment_Append_left_delta_star_split qi qf frag e1 e2 qf1 frag1 qf2 frag2 (qi + 1) frag.(frag_accept) s H REGEX1 REGEX2 RANGE1 DELTA eq_refl) as (s1 & s2 & EQ & DELTA1 & DELTA2).
+  pose proof (regex2fragment_Append_right_delta_star_split qi qf frag e1 e2 qf1 frag1 qf2 frag2 (qf1 + 1) frag.(frag_accept) s2 H REGEX1 REGEX2 RANGE2 DELTA2 eq_refl) as (s2' & s3 & EQ' & DELTA2' & DELTA3).
+  rewrite ACCEPT in DELTA3.
+  pose proof (regex2fragment_accept_delta_star_stuck (Re.Append e1 e2) qi qf frag qf s3 H DELTA3) as [EQ3 _].
+  subst s3. rewrite app_nil_r in EQ'. subst s2. subst s.
+  simpl. exists s1. split.
+  - eapply SOUND1; eauto. rewrite START1. rewrite ACCEPT1. exact DELTA1.
+  - exists s2'. split.
+    + eapply SOUND2; eauto. rewrite START2. rewrite ACCEPT2. exact DELTA2'.
+    + reflexivity.
+Qed.
+
+Theorem regex2fragment_sound_Star e1
+  (SOUND : forall qi, forall qf, forall frag, forall s, regex2fragment e1 qi = (qf, frag) -> frag.(frag_accept) \in fragment_delta_star frag frag.(frag_start) s -> s \in eval_regex e1)
+  : forall qi, forall qf, forall frag, forall s, regex2fragment (Re.Star e1) qi = (qf, frag) -> frag.(frag_accept) \in fragment_delta_star frag frag.(frag_start) s -> s \in eval_regex (Re.Star e1).
+Proof.
+  ii. pose proof (regex2fragment_Star_delta_star_start qi qf frag e1 s H H0) as (qf1 & frag1 & REGEX & DELTA).
+  pose proof (regex2fragment_bounds _ _ _ _ REGEX) as [START ACCEPT LT _ _].
+  assert (RANGE : qi + 1 <= qi + 1 <= qf1) by lia.
+  pose proof (regex2fragment_Star_delta_star_sound_aux e1 SOUND qi qf frag qf1 frag1 (qi + 1) frag.(frag_accept) s H REGEX RANGE DELTA eq_refl) as [[EQ _] | (s1 & s2 & EQ & DELTA1 & STAR)].
+  - subst s. simpl. econs.
+  - subst s. simpl. eapply star_app.
+    + eapply SOUND; eauto. rewrite START. rewrite ACCEPT. exact DELTA1.
+    + exact STAR.
+Qed.
+
+Corollary regex2fragment_sound e
+  : forall qi, forall qf, forall frag, forall s, regex2fragment e qi = (qf, frag) -> frag.(frag_accept) \in fragment_delta_star frag frag.(frag_start) s -> s \in eval_regex e.
+Proof.
+  induction e.
+  - now eapply regex2fragment_sound_Null.
+  - now eapply regex2fragment_sound_Empty.
+  - now eapply regex2fragment_sound_Char.
+  - now eapply regex2fragment_sound_Union.
+  - now eapply regex2fragment_sound_Append.
+  - now eapply regex2fragment_sound_Star.
+Qed.
+
+Lemma fragments_delta_star_start_to_fragment qi rules qmax frags rule frag qi_rule qf s
+  (FRAGS : rules2fragments qi rules = (qmax, frags))
+  (IN_FRAG : (rule, frag) ∈ frags)
+  (REGEX : regex2fragment rule.(Rule.regex) qi_rule = (qf, frag))
+  (qi_POS : 0 < qi)
+  (DELTA : frag.(frag_accept) \in fragments_delta_star frags 0 s)
+  : frag.(frag_accept) \in fragment_delta_star frag frag.(frag_start) s.
+Proof.
+  pose proof (regex2fragment_bounds _ _ _ _ REGEX) as [START ACCEPT LT _ _].
+  pose proof (delta_star_elim 0 frag.(frag_accept) s DELTA) as [NIL | [EPS | CHAR]].
+  - des; subst.
+    pose proof (rules2fragments_start_ge _ _ _ _ _ _ _ _ FRAGS IN_FRAG REGEX).
+    lia.
+  - destruct EPS as (q1 & STEP & REST).
+    pose proof (eps_step_from_edges_sound _ _ _ STEP) as IN_EDGE.
+    pose proof (fragment_eps_edges_start_sound _ _ _ _ _ FRAGS qi_POS IN_EDGE) as (rule' & frag' & qi_rule' & qf' & IN_FRAG' & REGEX' & START_EDGE).
+    subst q1.
+    pose proof (regex2fragment_bounds _ _ _ _ REGEX') as [START' ACCEPT' LT' _ _].
+    assert (RANGE : qi_rule <= frag.(frag_accept) <= qf) by lia.
+    assert (RANGE' : qi_rule' <= frag.(frag_accept) <= qf').
+    { eapply delta_star_fragment_range with (qi := qi) (rules := rules) (qmax := qmax) (frags := frags) (rule := rule') (frag := frag') (q := frag'.(frag_start)) (s := s); eauto. lia. }
+    pose proof (rules2fragments_ranges_disjoint _ _ _ _ _ _ _ _ _ _ _ _ _
+      FRAGS IN_FRAG IN_FRAG' REGEX REGEX' RANGE RANGE') as EQ.
+    inv EQ. eapply delta_star_global_to_fragment; eauto. lia.
+  - destruct CHAR as (c & s' & q1 & EQ & STEP & REST).
+    pose proof (char_step_from_edges_sound _ _ _ _ STEP) as (edge & IN_EDGE & SRC & LABEL & DST).
+    pose proof (fragment_char_edges_owner _ _ _ _ _ FRAGS IN_EDGE) as (rule' & frag' & qi_rule' & qf' & IN_FRAG' & REGEX' & BOUNDS' & LE_START & LT_END & RANGE' & IN_EDGE').
+    lia.
+Qed.
+
+Lemma TaggedENFA_FRAGMENTS_sound qi rules qmax frags s tag
+  (FRAGS : rules2fragments qi rules = (qmax, frags))
+  (qi_POS : 0 < qi)
+  (ACCEPTS : accepts (fragments2TaggedENFA qmax frags) s tag)
+  : exists rule, rule ∈ rules /\ rule.(Rule.token) = tag /\ s \in eval_regex rule.(Rule.regex).
+Proof.
+  destruct ACCEPTS as (q & DELTA & ACCEPT). simpl in DELTA, ACCEPT.
+  pose proof (fragment_accept_states_sound _ _ _ ACCEPT) as (rule & frag & IN_FRAG & ACCEPT_EQ & TOKEN_EQ); subst q tag.
+  pose proof (rules2fragments_bounds _ _ _ _ FRAGS) as [_ BOUND].
+  pose proof (BOUND _ _ IN_FRAG) as (qi_rule & qf & REGEX & _ & _ & _).
+  exists rule. split.
+  - eapply rules2fragments_sound; eauto.
+  - split; [reflexivity | ].
+    eapply regex2fragment_sound; eauto.
+    eapply fragments_delta_star_start_to_fragment; eauto.
+Qed.
+
+Theorem mkUnitedTaggedENFA_sound (M : TaggedENFA.t)
+  (COMPILE : fmap mkUnitedTaggedENFA Rule.compileds = inr M)
+  : exists rules, Rule.compileds = inr rules /\ ⟪ ACCEPT : forall s, forall tag, accepts M s tag -> (exists rule, rule ∈ rules /\ rule.(Rule.token) = tag /\ s \in eval_regex rule.(Rule.regex)) ⟫.
+Proof.
+  pose proof (mkUnitedTaggedENFA_spec M COMPILE) as (rules & qmax & frags & COMPILED & FRAGMENTS_OF).
+  destruct COMPILED as [COMPILED_RULES COMPILED_ENFA COMPILED_FRAGS].
+  exists rules. split; [exact COMPILED_RULES | unnw]. intros s tag ACCEPTS.
+  assert (ENFA_EQ : M = fragments2TaggedENFA qmax frags).
+  { eapply TaggedENFA_COMPILED_as_fragments. econs; eauto. }
+  rewrite ENFA_EQ in ACCEPTS. eapply TaggedENFA_FRAGMENTS_sound; eauto.
+Qed.
+
+Theorem mkUnitedTaggedENFA_complete (M : TaggedENFA.t)
+  (COMPILE : fmap mkUnitedTaggedENFA Rule.compileds = inr M)
+  : exists rules, Rule.compileds = inr rules /\ ⟪ ACCEPT : forall s, forall tag, (exists rule, rule ∈ rules /\ rule.(Rule.token) = tag /\ s \in eval_regex rule.(Rule.regex)) -> accepts M s tag ⟫.
+Proof.
+  pose proof (mkUnitedTaggedENFA_spec M COMPILE) as (rules & qmax & frags & COMPILED & FRAGMENTS_OF).
+  destruct COMPILED as [COMPILED_RULES COMPILED_ENFA COMPILED_FRAGS].
+  exists rules. split; [exact COMPILED_RULES | unnw]. intros s tag (rule & IN_RULE & TOKEN & IN_REGEX); subst tag.
+  pose proof (rules2fragments_complete 1 rules qmax frags rule COMPILED_FRAGS IN_RULE) as (qi & qf & frag & REGEX2FRAGMENT & IN_FRAGS).
+  pose proof (FRAGMENTS_OF rule frag IN_FRAGS) as FRAGMENTS.
+  pose proof (TaggedENFA_FRAGMENTS_complete qmax frags rule qi qf frag s REGEX2FRAGMENT FRAGMENTS IN_REGEX) as ACCEPTS.
+  rewrite TaggedENFA_COMPILED_as_fragments with (M := M) (rules := rules) (qmax := qmax) (frags := frags); eauto.
+  exact (TaggedENFA_COMPILED_intro M rules qmax frags COMPILED_RULES COMPILED_ENFA COMPILED_FRAGS).
+Qed.
+
+End Thompson's_construction.
+
+End TaggedENFA.
+
+Module DFA.
+
+#[projections(primitive)]
+Record t : Type :=
+  mk
+  { state : Set
+  ; state_hasEqDec : hasEqDec@{Set} state
+  ; states : list state
+  ; start_state : state
+  ; accept_states : list (state * Token.t)
+  ; transition (q : state) (c : ascii) : state
+  }.
+
+#[global] Existing Instance state_hasEqDec.
+
+Fixpoint delta (M : t) (q : M.(state)) (s : Input.t) {struct s} : M.(state) :=
+  match s with
+  | [] => q
+  | c :: s' => delta M (M.(transition) q c) s'
+  end.
+
+Definition accepts (M : t) (s : Input.t) (tag : Token.t) : Prop :=
+  (delta M M.(start_state) s, tag) ∈ M.(accept_states).
+
+Definition accepted_tags (M : t) (s : Input.t) : ensemble Token.t :=
+  fun tag => accepts M s tag.
+
+Section SUBSET_CONSTRUCTION.
+
+Variable M : TaggedENFA.t.
+
+#[local] Notation Q := M.(TaggedENFA.state).
+
+Definition subset_state : Set :=
+  list Q.
+
+Fixpoint iter {A : Type} (fuel : nat) (step : A -> A) (x : A) {struct fuel} : A :=
+  match fuel with
+  | O => x
+  | S fuel' => iter fuel' step (step x)
+  end.
+
+Definition normalize (qs : subset_state) : subset_state :=
+  filter (fun q => mem q qs) M.(TaggedENFA.states).
+
+Definition move (qs : subset_state) (c : ascii) : subset_state :=
+  qs >>= fun q => M.(TaggedENFA.char_step) q c.
+
+Definition eps_move (qs : subset_state) : subset_state :=
+  qs >>= M.(TaggedENFA.eps_step).
+
+Definition eclose_step (qs : subset_state) : subset_state :=
+  normalize (union (eps_move qs) qs).
+
+Definition eclose (qs : subset_state) : subset_state :=
+  iter (length M.(TaggedENFA.states)) eclose_step (normalize qs).
+
+Definition subset_states : list subset_state :=
+  powerset M.(TaggedENFA.states).
+
+Definition subset_start_state : subset_state :=
+  eclose [M.(TaggedENFA.start_state)].
+
+Definition subset_transition (qs : subset_state) (c : ascii) : subset_state :=
+  eclose (move qs c).
+
+Definition subset_accept_states_of (qs : subset_state) : list (subset_state * Token.t) :=
+  M.(TaggedENFA.accept_states) >>= fun '(q, tag) => if mem q qs then [(qs, tag)] else [].
+
+Definition subset_accept_states : list (subset_state * Token.t) :=
+  subset_states >>= subset_accept_states_of.
+
+Definition subset_construct : DFA.t :=
+  {|
+    state := subset_state;
+    state_hasEqDec := list_hasEqDec M.(TaggedENFA.state_hasEqDec);
+    states := subset_states;
+    start_state := subset_start_state;
+    accept_states := subset_accept_states;
+    transition := subset_transition;
+  |}.
+
+End SUBSET_CONSTRUCTION.
+
+Section MINIMISATION.
+
+Variable M : DFA.t.
+
+#[local] Notation Q := M.(state).
+
+Definition accepts_from (q : Q) (s : Input.t) (tag : Token.t) : Prop :=
+  (delta M q s, tag) ∈ M.(accept_states).
+
+Definition accepting_tags_from (q : Q) : list Token.t :=
+  M.(accept_states) >>= fun '(q', tag) => if eq_dec q q' then [tag] else [].
+
+Definition same_accepting_tagsb (q1 : Q) (q2 : Q) : bool :=
+  forallb (fun '(_, tag) => eqb (mem (q1, tag) M.(accept_states)) (mem (q2, tag) M.(accept_states))) M.(accept_states).
+
+Fixpoint minimisation_equivb (fuel : nat) (q1 : Q) (q2 : Q) {struct fuel} : bool :=
+  match fuel with
+  | O => same_accepting_tagsb q1 q2
+  | S fuel' => same_accepting_tagsb q1 q2 && forallb (fun c => minimisation_equivb fuel' (M.(transition) q1 c) (M.(transition) q2 c)) all_asciis
+  end.
+
+Definition minimisation_equiv (q1 : Q) (q2 : Q) : Prop :=
+  minimisation_equivb (length M.(states)) q1 q2 = true.
+
+Definition minimised_state : Set :=
+  list Q.
+
+Definition minimisation_class (q : Q) : minimised_state :=
+  filter (minimisation_equivb (length M.(states)) q) M.(states).
+
+Definition minimised_states : list minimised_state :=
+  map minimisation_class M.(states).
+
+Definition representative (qs : minimised_state) : Q :=
+  match qs with
+  | [] => M.(start_state)
+  | q :: _ => q
+  end.
+
+Definition minimised_start_state : minimised_state :=
+  minimisation_class M.(start_state).
+
+Definition minimised_transition (qs : minimised_state) (c : ascii) : minimised_state :=
+  minimisation_class (M.(transition) (representative qs) c).
+
+Definition minimised_accept_states_of (qs : minimised_state) : list (minimised_state * Token.t) :=
+  accepting_tags_from (representative qs) >>= fun tag => [(qs, tag)].
+
+Definition minimised_accept_states : list (minimised_state * Token.t) :=
+  minimised_states >>= minimised_accept_states_of.
+
+Definition minimise : DFA.t :=
+  {|
+    state := minimised_state;
+    state_hasEqDec := list_hasEqDec M.(state_hasEqDec);
+    states := minimised_states;
+    start_state := minimised_start_state;
+    accept_states := minimised_accept_states;
+    transition := minimised_transition;
+  |}.
+
+End MINIMISATION.
+
+Section DELETE_DEAD_STATE.
+
+Variable M : DFA.t.
+
+#[local] Notation Q := M.(state).
+
+Definition delete_state_set : Set :=
+  list Q.
+
+Definition delete_normalize (qs : delete_state_set) : delete_state_set :=
+  filter (fun q => mem q qs) M.(states).
+
+Definition delete_successors (q : Q) : delete_state_set :=
+  map (M.(transition) q) all_asciis.
+
+Definition delete_reachable_move (qs : delete_state_set) : delete_state_set :=
+  qs >>= delete_successors.
+
+Definition delete_reachable_step (qs : delete_state_set) : delete_state_set :=
+  delete_normalize (union (delete_reachable_move qs) qs).
+
+Definition reachable_states : delete_state_set :=
+  iter (length M.(states)) delete_reachable_step (delete_normalize [M.(start_state)]).
+
+Definition accepting_stateb (q : Q) : bool :=
+  existsb (fun '(q', _) => eqb q q') M.(accept_states).
+
+Definition accepting_states : delete_state_set :=
+  filter accepting_stateb M.(states).
+
+Definition predecessorb (q : Q) (p : Q) : bool :=
+  existsb (fun c => eqb (M.(transition) p c) q) all_asciis.
+
+Definition predecessors (q : Q) : delete_state_set :=
+  filter (predecessorb q) M.(states).
+
+Definition live_move (qs : delete_state_set) : delete_state_set :=
+  qs >>= predecessors.
+
+Definition live_step (qs : delete_state_set) : delete_state_set :=
+  delete_normalize (union (live_move qs) qs).
+
+Definition live_states : delete_state_set :=
+  iter (length M.(states)) live_step accepting_states.
+
+Definition dead_states : delete_state_set :=
+  filter (fun q => negb (mem q live_states)) M.(states).
+
+Definition useful_states : delete_state_set :=
+  filter (fun q => mem q reachable_states && mem q live_states) M.(states).
+
+Definition delete_dead_accept_states : list (Q * Token.t) :=
+  filter (fun '(q, _) => mem q live_states) M.(accept_states).
+
+Definition delete_dead_state : DFA.t :=
+  {|
+    state := Q;
+    state_hasEqDec := M.(state_hasEqDec);
+    states := live_states;
+    start_state := M.(start_state);
+    accept_states := delete_dead_accept_states;
+    transition := M.(transition);
+  |}.
+
+End DELETE_DEAD_STATE.
+
+End DFA.
+
+Definition t : Type :=
+  DFA.t.
+
+Fixpoint first_accepting_token_from {Q : Set} `{Q_hasEqDec : hasEqDec@{Set} Q} (q : Q) (accept_states : list (Q * Token.t)) {struct accept_states} : option Token.t :=
+  match accept_states with
+  | [] => None
+  | (q', tag) :: accept_states' => if eq_dec q q' then Some tag else first_accepting_token_from q accept_states'
+  end.
+
+Definition first_accepting_token (M : LGS.t) (q : M.(DFA.state)) : option Token.t :=
+  @first_accepting_token_from M.(DFA.state) M.(DFA.state_hasEqDec) q M.(DFA.accept_states).
+
+Fixpoint maximal_munch (M : LGS.t) (q : M.(DFA.state)) (s : list ascii) (best : option (list ascii * Token.t)) {struct s} : option (list ascii * Token.t) :=
+  match s with
+  | [] => best
+  | c :: s' =>
+    let q' := M.(DFA.transition) q c in
+    let best' := B.maybe (A := _) (B := fun _ => _) best (fun tag => Some (s', tag)) (first_accepting_token M q') in
+    maximal_munch M q' s' best'
+  end.
+
+Definition scan_one (M : t) (s : list ascii) : option (list ascii * Token.t) :=
+  maximal_munch M M.(DFA.start_state) s None.
+
+Definition input_lt (s1 : Input.t) (s2 : Input.t) : Prop :=
+  length s1 < length s2.
+
+Fixpoint scan_all' (M : LGS.t) (s : list ascii) (H_Acc : Acc input_lt s) {struct H_Acc} : option (list Token.t) :=
+  if L.null s then
+    Some []
+  else
+    match scan_one M s with
+    | None => None
+    | Some (rest, tag) =>
+      match lt_dec (length rest) (length s) with
+      | left LT =>
+        match scan_all' M rest (Acc_inv H_Acc rest LT) with
+        | None => None
+        | Some tags => Some (tag :: tags)
+        end
+      | right _ => None
+      end
+    end.
+
+Definition scan_all (M : LGS.t) (s : list ascii) : option (list Token.t) :=
+  scan_all' M s (L.length_lt_wf s).
+
+Definition build : BuildErrorM LGS.t := do
+  'rules <- Rule.compileds;
+  ret (DFA.delete_dead_state (DFA.minimise (DFA.subset_construct (TaggedENFA.mkUnitedTaggedENFA rules))))
+  end. 
 
 End LGS.
